proof/access-control/RISCV64/ArchCNode_AC.thy
@@ -347,752 +347,252 @@ qed
 
 context Arch begin global_naming RISCV64
 
-lemma pas_refined_arch_state_update_not_asids[simp]:
- "riscv_asid_table (f (arch_state s)) = riscv_asid_table (arch_state s)
-  \<Longrightarrow> pas_refined aag (arch_state_update f s) = pas_refined aag s"
-  apply (auto simp add: pas_refined_def state_objs_to_policy_def)
-apply (erule subsetD)
-  oops
-
-crunch cdt[wp]: store_pte "\<lambda>s. P (cdt s)"
-
-lemma store_pte_state_refs[wp]:
-  "store_pte p pte \<lbrace>\<lambda>s. P (state_refs_of s)\<rbrace>"
-  apply (simp add: store_pte_def set_pt_def set_object_def)
-  apply (wp get_object_wp)
-  apply (clarsimp simp: obj_at_def state_refs_of_def
-                 elim!: rsubst[where P=P, OF _ ext])
-  done
-
-(* FIXME ryanb - remove? *)
-lemma all_rsubst:
-  "\<lbrakk> \<forall>v. P (f v); \<exists>v. f v = r \<rbrakk> \<Longrightarrow> P r"
-  by clarsimp
-
-
-
-lemma "\<lbrace>valid_pti pti\<rbrace> perform_page_table_invocation pti \<lbrace>Q\<rbrace>"
-apply (unfold perform_page_table_invocation_def perform_pt_inv_map_def perform_pt_inv_unmap_def)
-apply (case_tac pti; clarsimp simp: valid_pti_def)
-apply (rename_tac acap cslot_a cslot_b pte pt_slot)
-thm valid_vspace_objs_def
-term wellformed_pte
-term perform_page_table_invocation
-term perform_pt_inv_map
-term valid_pti
-term invalid_pte_at
-oops
-
-lemma "\<lbrace>valid_pti pti\<rbrace> perform_page_table_invocation pti \<lbrace>Q\<rbrace>"
-apply (unfold perform_page_table_invocation_def perform_pt_inv_map_def perform_pt_inv_unmap_def)
-apply (case_tac pti; clarsimp simp: valid_pti_def)
-subgoal sorry
-apply (rename_tac acap cslot_a cslot_b)
-thm valid_vspace_objs_def
-term wellformed_pte
-term perform_page_table_invocation
-term perform_pt_inv_map
-term valid_pti
-term invalid_pte_at
-oops
-
-
-
-lemma vs_lookup_PageTablePTE:
-  "\<lbrakk> pspace_aligned s; valid_vspace_objs s; valid_asid_table s;
-     invalid_pte_at p s; ptes_of s' = ptes_of s (p \<mapsto> pte); is_PageTablePTE pte;
-     asid_pools_of s' = asid_pools_of s; asid_table s' = asid_table s;
-     vref \<in> user_region; vs_lookup_table level asid vref s' = Some (lvl', pt);
-     pts_of s (the (pte_ref pte)) = Some empty_pt; pt \<noteq> pptr_from_pte pte \<rbrakk>
-     \<Longrightarrow> \<exists>level' \<ge> level. vs_lookup_table level' asid vref s = Some (lvl', pt)"
-  apply (induct level arbitrary: lvl' pt rule: bit0.from_top_full_induct[where y=max_pt_level])
-   apply (fastforce simp: geq_max_pt_level vs_lookup_table_def pool_for_asid_def obind_def)
-  apply (rule_tac x=lvl' in exI)
-  apply (rule context_conjI)
-   apply (fastforce dest: vs_lookup_min_level)
-  apply (drule vs_lookup_level)
-  apply (case_tac "lvl' < max_pt_level")
-   apply (frule vs_lookup_table_split_last_Some; clarsimp)
-   apply (erule_tac x="lvl'+1" in allE)
-   apply (drule mp)
-    apply (fastforce elim: le_less_trans dest: vm_level_less_plus_1_mono)
-   apply (erule_tac x="lvl'+1" in allE)
-   apply clarsimp
-   apply (frule subst[where s="ptes_of s'" and P="\<lambda>ptes. ptes _ = _"])
-    apply assumption
-   apply (drule mp, fastforce simp: pte_ref_def2 ptes_of_Some split: if_splits)
-   apply (cases pte; clarsimp)
-   apply (drule_tac bot_level=level' in vs_lookup_level)
-   apply (subst vs_lookup_split_Some)
-     prefer 3
-     apply (rule exI, rule conjI, assumption)
-     apply (frule_tac P="\<lambda>x. x" and level1=lvl' and level'1="lvl'+1"
-                   in subst[OF vs_lookup_split_Some, rotated 2])
-       apply (fastforce dest: vm_level_less_le_1)
-      apply (fastforce dest: vm_level_less_max_pt_level vm_level_less_plus_1_mono)
-     apply clarsimp
-     apply (subst (asm) pt_walk.simps)
-     apply (clarsimp simp: obind_def)
-     apply (subst pt_walk.simps)
-     apply (clarsimp split: if_splits simp: obind_def)
-    apply (fastforce dest: vm_level_less_le_1)
-   apply (fastforce dest: vm_level_less_max_pt_level vm_level_less_plus_1_mono)
-  apply (case_tac "lvl' = asid_pool_level")
-   apply (auto simp: geq_max_pt_level vs_lookup_table_def pool_for_asid_def obind_def)
-  done
-
-lemma vs_lookup_PageTablePTE':
-  "\<lbrakk> pspace_aligned s; valid_vspace_objs s; valid_asid_table s;
-     invalid_pte_at p s; ptes_of s' = ptes_of s (p \<mapsto> pte); is_PageTablePTE pte;
-     asid_pools_of s' = asid_pools_of s; asid_table s' = asid_table s;
-     vref \<in> user_region; vs_lookup_table level asid vref s = Some (lvl', pt) \<rbrakk>
-     \<Longrightarrow> \<exists>level' \<ge> level. vs_lookup_table level' asid vref s' = Some (lvl', pt)"
-  apply (induct level arbitrary: lvl' pt rule: bit0.from_top_full_induct[where y=max_pt_level])
-   apply (fastforce simp: geq_max_pt_level vs_lookup_table_def pool_for_asid_def obind_def)
-  apply (rule_tac x=lvl' in exI)
-  apply (rule context_conjI)
-   apply (fastforce dest: vs_lookup_min_level)
-  apply (drule vs_lookup_level)
-  apply (case_tac "lvl' < max_pt_level")
-   apply (frule vs_lookup_table_split_last_Some; clarsimp)
-   apply (erule_tac x="lvl'+1" in allE)
-   apply (drule mp)
-    apply (fastforce elim: le_less_trans dest: vm_level_less_plus_1_mono)
-   apply (erule_tac x="lvl'+1" in allE)
-   apply clarsimp
-   apply (drule_tac bot_level=level' in vs_lookup_level)
-   apply (subst vs_lookup_split_Some)
-     prefer 3
-     apply (rule exI, rule conjI, assumption)
-     apply (frule_tac P="\<lambda>x. x" and level1=lvl' and level'1="lvl'+1"
-                   in subst[OF vs_lookup_split_Some, rotated 2])
-       apply (fastforce dest: vm_level_less_le_1)
-      apply (fastforce dest: vm_level_less_max_pt_level vm_level_less_plus_1_mono)
-     apply clarsimp
-     apply (subst (asm) pt_walk.simps)
-     apply (clarsimp simp: obind_def split: if_splits)
-     apply (subst pt_walk.simps)
-     apply (clarsimp simp: obind_def split: if_splits)
-     apply (cases pte; clarsimp)
-     apply (frule is_aligned_pt[rotated])
-      apply (erule vs_lookup_table_pt_at; fastforce)
-     apply (clarsimp simp: invalid_pte_at_def ptes_of_Some pts_of_Some aobjs_of_Some)
-    apply (fastforce dest: vm_level_less_le_1)
-   apply (fastforce dest: vm_level_less_max_pt_level vm_level_less_plus_1_mono)
-  apply (case_tac "lvl' = asid_pool_level")
-   apply (auto simp: geq_max_pt_level vs_lookup_table_def pool_for_asid_def obind_def)
-  done
-
-
-lemma vs_lookup_slot_table_base':
-  "\<lbrakk> vs_lookup_slot level asid vref s = Some (level, slot); vref \<in> user_region;
-     level \<le> max_pt_level; invs s \<rbrakk> \<Longrightarrow>
-   slot = pt_slot_offset level (table_base slot) vref"
-  apply (clarsimp simp: vs_lookup_slot_def split: if_split_asm)
-  apply (drule vs_lookup_table_is_aligned; clarsimp)
-  done
-
-
-lemma level_of_slot_vs_lookup_slot:
+lemma vs_lookup_slot_level_of_slot:
   "\<lbrakk> vs_lookup_slot level asid vref s = Some (level, p);
      ptes_of s p = Some pte; level \<le> max_pt_level; vref \<in> user_region; invs s \<rbrakk>
      \<Longrightarrow> level_of_slot asid vref p s = level"
-apply (subst level_of_slot_def)
-apply (rule Greatest_equality)
-apply clarsimp
-thm vs_lookup_slot_no_asid vs_lookup_slot_unique_level
-    apply (case_tac "y = asid_pool_level")
-apply clarsimp
-apply (drule vs_lookup_slot_no_asid)
-apply simp
-apply clarsimp+
+  apply (subst level_of_slot_def)
+  apply (rule Greatest_equality)
+   apply clarsimp
+  apply (case_tac "y = asid_pool_level")
+   apply (fastforce dest: vs_lookup_slot_no_asid)
+  apply (fastforce dest: vs_lookup_slot_unique_level)
+  done
 
-apply (drule (1) vs_lookup_slot_unique_level)
-apply fastforce+
-done
+lemma state_vrefsD:
+  "\<lbrakk> vs_lookup_table level asid vref s = Some (lvl, p);
+     aobjs_of s p = Some ao; vref \<in> user_region; x \<in> vs_refs_aux lvl ao \<rbrakk>
+     \<Longrightarrow> x \<in> state_vrefs s p"
+  unfolding state_vrefs_def by fastforce
 
+lemma pool_for_asid_vs_lookupD:
+  "pool_for_asid asid s = Some p \<Longrightarrow>
+   vs_lookup_table asid_pool_level asid vref s = Some (asid_pool_level, p)"
+  by (simp add: pool_for_asid_vs_lookup)
+
+lemma vs_lookup_table_vref_independent:
+  "\<lbrakk> vs_lookup_table level asid vref s = opt; level \<ge> max_pt_level \<rbrakk>
+     \<Longrightarrow> vs_lookup_table level asid vref' s = opt"
+  by (cases "level = asid_pool_level"; clarsimp simp: vs_lookup_table_def)
 
 lemma state_vrefs_store_NonPageTablePTE:
   "\<lbrakk> invs s; is_aligned p pte_bits; vs_lookup_slot level asid vref s = Some (level, p);
      vref \<in> user_region; \<not> is_PageTablePTE pte;
      kheap s (table_base p) = Some (ArchObj (PageTable pt)) \<rbrakk>
      \<Longrightarrow> state_vrefs (s\<lparr>kheap := \<lambda>a. if a = table_base p
-                                     then Some (ArchObj (PageTable (\<lambda>a. if a = table_index p then pte else pt a)))
+                                     then Some (ArchObj (PageTable (\<lambda>a. if a = table_index p
+                                                                        then pte
+                                                                        else pt a)))
                                      else kheap s a\<rparr>) =
-         (\<lambda>x. if \<exists>level' vref'. vref' \<in> user_region \<and> vref_for_level vref' (level + 1) = vref_for_level vref (level + 1) \<and>
-                                p = pt_slot_offset level (table_base p) vref' \<and>
+         (\<lambda>x. if \<exists>level' vref'. vref_for_level vref' (level + 1) = vref_for_level vref (level + 1) \<and>
+                                vref' \<in> user_region \<and> p = pt_slot_offset level (table_base p) vref' \<and>
                                 pt_walk level level' (table_base p) vref' (ptes_of s) = Some (level',x)
               then (if x = table_base p
                     then vs_refs_aux level (PageTable (\<lambda>a. if a = table_index p then pte else pt a))
                     else {})
               else state_vrefs s x)"
   apply (rule all_ext)
-
   apply (case_tac "level = asid_pool_level")
-   apply (clarsimp simp: vs_lookup_slot_def split: if_splits)
-   apply (clarsimp simp: vs_lookup_table_def split: if_splits)
-   apply (drule pool_for_asid_no_pte)
-      apply (simp add: ptes_of_Some pts_of_Some aobjs_of_Some)
-     apply fastforce
-    apply fastforce
-   apply fastforce
-
-apply (prop_tac "ptes_of s p \<noteq> None")
-apply (drule valid_vspace_objs_strong_slotD)
-apply fastforce+
-
-  apply (frule vs_lookup_slot_table_base')
-     apply fastforce+
-  apply (drule vs_lookup_slot_table_base)
-     apply fastforce+
-
+   apply (fastforce simp: vs_lookup_slot_def vs_lookup_table_def
+                          ptes_of_Some pts_of_Some aobjs_of_Some
+                    dest: pool_for_asid_no_pte)
+  apply (prop_tac "ptes_of s p \<noteq> None")
+   apply (drule valid_vspace_objs_strong_slotD; clarsimp split del: if_split)
+  apply (frule vs_lookup_slot_table_base; clarsimp split del: if_split)
+  apply (subst (asm) vs_lookup_slot_table_unfold; clarsimp split del: if_split)
   apply safe
-
-
-(* first thing *)
    apply (subst (asm) state_vrefs_def opt_map_def)+
    apply (clarsimp split: option.splits split del: if_split)
-   apply (clarsimp split: if_split_asm option.splits split del: if_split)
-(* x = table_base p *)
-    apply (subst (asm) vs_lookup_non_PageTablePTE[where s=s and p=p and pte=pte])
-           apply (clarsimp simp: ptes_of_Some pts_of_Some aobjs_of_Some)
-          apply (rule all_ext)
-          apply (clarsimp simp: opt_map_def pte_of_def obind_def)
-          apply (fastforce dest: pte_ptr_eq)
-         apply simp
-        apply (fastforce simp: opt_map_def)
-       apply (fastforce simp: opt_map_def)
-      apply fastforce+
-    (* done *)
-
-    apply (clarsimp split: if_splits)
-
-
-     apply (rule conjI)
-      prefer 2
-      apply clarsimp
-      apply (erule_tac x=level in allE)
-      apply (erule_tac x=vref in allE)
-      apply clarsimp
-
-     apply (drule vs_lookup_level) back
-
-     apply (case_tac "lvl = asid_pool_level")
-      apply clarsimp
-      apply (frule vs_lookup_table_no_asid)
-         apply (fastforce simp: ptes_of_Some pts_of_Some aobjs_of_Some)
-        apply fastforce
-       apply fastforce
-      apply fastforce
-
-     apply clarsimp
-     apply (drule (1) vs_lookup_table_unique_level)
-           apply fastforce+
-
-    apply (rule conjI)
-     prefer 2
-     apply clarsimp
-     apply (erule_tac x=level in allE) back
-     apply clarsimp
-
-     apply (drule vs_lookup_level) back
-
-     apply (case_tac "lvl = asid_pool_level")
-      apply clarsimp
-      apply (frule vs_lookup_table_no_asid)
-         apply (fastforce simp: ptes_of_Some pts_of_Some aobjs_of_Some)
-        apply fastforce
-       apply fastforce
-      apply fastforce
-
-     apply clarsimp
-     apply (drule (1) vs_lookup_table_unique_level)
-           apply fastforce+
-(* x \<noteq> table_base p *)
-
-
-   apply (subst (asm) vs_lookup_non_PageTablePTE[where s=s and p=p and pte=pte])
-          apply (clarsimp simp: ptes_of_Some pts_of_Some aobjs_of_Some)
-         apply (rule all_ext)
-         apply (clarsimp simp: opt_map_def pte_of_def obind_def)
-         apply (fastforce dest: pte_ptr_eq)
-        apply simp
-       apply (fastforce simp: opt_map_def)
-      apply (fastforce simp: opt_map_def)
-     apply fastforce+
-    (* done *)
-
-   apply (subst state_vrefs_def)
-   apply (clarsimp split: if_splits)
-
-  apply (case_tac "level' = asid_pool_level")
-      apply clarsimp
-      apply (frule vs_lookup_slot_no_asid)
-         apply (fastforce simp: ptes_of_Some pts_of_Some aobjs_of_Some)
-        apply fastforce
-       apply fastforce
-      apply fastforce
-    apply clarsimp
-
-    apply (prop_tac "level_of_slot asida vrefa p s = level'")
-apply (erule level_of_slot_vs_lookup_slot)
-apply (fastforce simp: ptes_of_Some pte_of_def obind_def pts_of_Some aobjs_of_Some split: option.splits)
-apply fastforce+
-
-    apply (subst (asm) vs_lookup_slot_table_unfold; fastforce)
-
-   apply (rule conjI)
-    prefer 2
-    apply (fastforce simp: opt_map_def)
-   apply clarsimp
-
-
-   apply (case_tac "level' < level")
-    prefer 2
-    apply (subst (asm) pt_walk.simps)
-    apply clarsimp
-
-
-apply (prop_tac "vs_lookup_slot level asid vref s = Some (level, p)")
-apply (fastforce simp: vs_lookup_slot_table_unfold)
-
-
-   apply (subst (asm) vs_lookup_vref_for_level_eq1)
-    apply (rule sym)
-    apply assumption
-
-
-   apply (frule (2) vs_lookup_table_extend)
-
-   apply (frule vs_lookup_min_level) back
-   apply (drule vs_lookup_level) back
-
-
+   apply (subst (asm) vs_lookup_non_PageTablePTE[where s=s and s'="kheap_update _ s" and p=p])
+          apply (fastforce simp: ptes_of_Some pts_of_Some aobjs_of_Some
+                                 opt_map_def pte_of_def obind_def
+                           dest: pte_ptr_eq)+
+   apply (case_tac "x = table_base p"; clarsimp)
     apply (case_tac "lvl = asid_pool_level")
-     apply (drule vs_lookup_table_pt_at) back
-          apply fastforce+
-         apply clarsimp
-         apply (frule vs_lookup_asid_pool)
-          apply fastforce
-         apply (clarsimp simp: asid_pools_of_ko_at obj_at_def)
-
-         apply (drule (1) vs_lookup_table_unique_level, rule refl)
-         apply fastforce+
-
-         apply clarsimp
-         apply (prop_tac "level' + 1 \<le> level")
-          apply (fastforce simp: bit0.plus_one_leq)
-
-
-         apply (erule_tac x=level in allE)
-         apply (drule mp)
-
-          apply (subst vs_lookup_slot_vref_for_level[symmetric])
-           apply assumption
-          apply (simp only:)
-          apply (subst vs_lookup_slot_vref_for_level)
-           apply assumption
-          apply (fastforce simp: vs_lookup_slot_table_unfold)
-          apply fastforce
-
-
-(* second bit *)
-
-apply (clarsimp simp: obind_def split: if_splits option.splits)
-
-(* second thing *)
-
-  apply (clarsimp simp: state_vrefs_def opt_map_def)
-
-apply (intro exI conjI)
-apply (rule refl)
-apply (subst vs_lookup_non_PageTablePTE[where s=s and p=p and pte=pte ])
-apply (clarsimp simp: ptes_of_Some pts_of_Some aobjs_of_Some)
- apply (rule all_ext)
-        apply (clarsimp simp: opt_map_def pte_of_def obind_def)
-        apply (fastforce dest: pte_ptr_eq)
-       apply simp
-      apply (fastforce simp: opt_map_def)
-     apply (fastforce simp: opt_map_def)
-    apply fastforce
-    apply fastforce
-defer
-apply fastforce
-apply fastforce
-apply fastforce
-defer
-apply (clarsimp split: if_splits)
-apply auto[1]
-
-
-apply (prop_tac "level_of_slot asid vref p s = level")
-apply (subst level_of_slot_def)
-
-apply (rule Greatest_equality)
-apply (clarsimp simp: vs_lookup_slot_def obind_def)
-
- apply (case_tac "ya = asid_pool_level")
-    (* lvla = asid_pool_level *)
-    apply clarsimp
-    apply (frule vs_lookup_slot_no_asid)
-         apply (clarsimp simp: ptes_of_Some pts_of_Some aobjs_of_Some pte_of_def obind_def split: option.splits)
-apply fastforce
-apply fastforce
-apply fastforce
-apply clarsimp
-apply clarsimp
-
-apply (subst (asm) vs_lookup_slot_table_unfold) back
-apply fastforce+
-
-apply clarsimp
-apply (drule (1) vs_lookup_table_unique_level)
-apply fastforce+
-
-apply (clarsimp simp: state_vrefs_def)
-apply (subst opt_map_def)
-apply (case_tac "x = table_base p"; clarsimp)
-
-apply (rule exI, rule conjI)
-prefer 2
-apply assumption
-apply (rule exI)+
-apply (rule conjI, rule refl)
-apply (clarsimp simp: aobjs_of_Some)
-apply (erule_tac x=level in allE)
-apply (erule_tac x=vref in allE)
-apply clarsimp
-
-apply (rule exI, rule conjI)
-prefer 2
-apply assumption
-apply (rule exI)+
-apply (rule conjI, rule refl)
-apply (clarsimp simp: aobjs_of_Some)
-
-apply (case_tac "lvl < level")
-
-apply (drule vs_lookup_level) back
-apply (subst (asm) vs_lookup_split_Some[where level'=level]) back
-apply fastforce
-apply fastforce
-apply clarsimp
-
-apply (rule_tac x=lvl in exI)
-apply (rule_tac x=asida in exI)
-apply (rule_tac x=vrefa in exI)
-
-
-apply (subst vs_lookup_non_PageTablePTE[where s=s and p=p and pte=pte ])
-apply (clarsimp simp: ptes_of_Some pts_of_Some aobjs_of_Some)
- apply (rule all_ext)
-        apply (clarsimp simp: opt_map_def pte_of_def obind_def)
-        apply (fastforce dest: pte_ptr_eq)
-       apply simp
-      apply (fastforce simp: opt_map_def)
-     apply (fastforce simp: opt_map_def)
-    apply fastforce
-    apply fastforce
-  apply (clarsimp split: if_splits)
-  apply (intro conjI; clarsimp)
-prefer 2
-  using vs_lookup_table_extend apply blast
-
+     apply (fastforce dest: vs_lookup_table_no_asid[OF vs_lookup_level]
+                      simp: ptes_of_Some pts_of_Some aobjs_of_Some split: if_splits)
+    apply (fastforce dest: vs_lookup_table_unique_level[OF vs_lookup_level]
+                     elim: allE[where x=level] split: if_splits)
+   apply (clarsimp split: if_splits)
     apply (case_tac "level' = asid_pool_level")
-     apply (fastforce dest: vs_lookup_slot_no_asid
-                       simp: ptes_of_Some pts_of_Some aobjs_of_Some pte_of_def obind_def split: option.splits)
+     apply (fastforce dest: vs_lookup_slot_no_asid simp: ptes_of_Some pts_of_Some aobjs_of_Some)
+    apply (frule vs_lookup_slot_level_of_slot)
+        apply (fastforce simp: ptes_of_Some pts_of_Some aobjs_of_Some split: option.splits)
+       apply fastforce+
+    apply (subst (asm) vs_lookup_slot_table_unfold; fastforce)
+   apply (rule conjI; clarsimp)
+    apply (case_tac "level' < level")
+     apply (subst (asm) vs_lookup_vref_for_level_eq1, rule sym, assumption)
+     apply (frule (2) vs_lookup_table_extend)
+     apply (case_tac "lvl = asid_pool_level")
+      apply (fastforce dest: vs_lookup_table_pt_at vs_lookup_asid_pool
+                       simp: asid_pools_of_ko_at obj_at_def)
+     apply (frule_tac level=lvl in vs_lookup_level)
+     apply (drule (1) vs_lookup_table_unique_level, rule refl)
+          apply fastforce+
+     apply (frule bit0.plus_one_leq)
+     apply (erule_tac x=level in allE)
+     apply (subst (asm) vs_lookup_slot_vref_for_level[symmetric], assumption)
+     apply (frule_tac bot_level=bot in vs_lookup_min_level)
+     apply (fastforce simp: vs_lookup_slot_vref_for_level vs_lookup_slot_table_unfold)
+    apply (subst (asm) pt_walk.simps, clarsimp)
+   apply (fastforce simp: state_vrefs_def opt_map_def)
+  apply (prop_tac "level_of_slot asid vref p s = level")
+   apply (fastforce simp: vs_lookup_slot_table_unfold vs_lookup_slot_level_of_slot)
+  apply (clarsimp split: if_splits)
+   apply (rule state_vrefsD)
+      apply (subst vs_lookup_non_PageTablePTE[where s=s and p=p and pte=pte])
+             apply (fastforce dest: pte_ptr_eq
+                              simp: ptes_of_Some pts_of_Some aobjs_of_Some
+                                    opt_map_def pte_of_def obind_def)+
+  apply (case_tac "x = table_base p")
+   apply (fastforce elim: allE[where x=level])
+  apply (subst (asm) state_vrefs_def, clarsimp)
+  apply (rule_tac level=lvl and asid=asida and vref=vrefa in state_vrefsD)
+     apply (subst vs_lookup_non_PageTablePTE[where s=s and p=p and pte=pte])
+            apply (fastforce dest: pte_ptr_eq
+                             simp: ptes_of_Some pts_of_Some aobjs_of_Some
+                                   opt_map_def pte_of_def obind_def)+
+     apply (clarsimp split: if_splits)
+     apply (intro conjI; clarsimp)
+      apply (case_tac "level' = asid_pool_level")
+       apply (fastforce dest: vs_lookup_slot_no_asid simp: ptes_of_Some pts_of_Some aobjs_of_Some)
+      apply (subst (asm) vs_lookup_slot_table_unfold; clarsimp)
+      apply (case_tac "lvl < level")
+       apply (drule_tac bot_level=bot in vs_lookup_level)
+       apply (subst (asm) vs_lookup_split_Some, erule dual_order.strict_implies_order)
+        apply fastforce
+       apply (drule (1) vs_lookup_table_unique_level; fastforce)
+      apply (metis vs_lookup_slot_table vs_lookup_slot_unique_level)
+     apply (fastforce dest: vs_lookup_level)
+    apply (fastforce simp: aobjs_of_Some opt_map_def)
    apply clarsimp
+  apply clarsimp
+  done
 
-apply (prop_tac "level_of_slot asida vrefa p s = level'")
-
-apply (subst level_of_slot_def)
-apply (rule Greatest_equality)
-apply clarsimp
-
-    apply (case_tac "ya = asid_pool_level")
-     apply (fastforce dest: vs_lookup_slot_no_asid
-                       simp: ptes_of_Some pts_of_Some aobjs_of_Some pte_of_def obind_def split: option.splits)
-   apply clarsimp
-
-apply (drule (1) vs_lookup_slot_unique_level)
-apply fastforce+
-
-apply (simp only:)
-apply (thin_tac "level_of_slot _ _ _ _ = _")
-
-apply (subst (asm) vs_lookup_slot_table_unfold)
-apply fastforce+
-apply clarsimp
-apply (drule (1) vs_lookup_table_unique_level) back
-apply fastforce+
-
-
-apply (rule_tac x=lvl in exI)
-apply (rule_tac x=asida in exI)
-apply (rule_tac x=vrefa in exI)
-apply clarsimp
-
-
-apply (subst vs_lookup_non_PageTablePTE[where s=s and p=p and pte=pte ])
-apply (clarsimp simp: ptes_of_Some pts_of_Some aobjs_of_Some)
- apply (rule all_ext)
-        apply (clarsimp simp: opt_map_def pte_of_def obind_def)
-        apply (fastforce dest: pte_ptr_eq)
-       apply simp
-      apply (fastforce simp: opt_map_def)
-     apply (fastforce simp: opt_map_def)
-    apply fastforce
-    apply fastforce
-apply (case_tac "\<exists>level'. vs_lookup_slot level' asida vrefa s = Some (level', p) \<and> lvl < level'"; clarsimp)
-
-prefer 2
-apply (fastforce dest: vs_lookup_level)
-apply (case_tac "level' = asid_pool_level")
-apply clarsimp
-apply (frule vs_lookup_slot_no_asid)
-         apply (clarsimp simp: ptes_of_Some pts_of_Some aobjs_of_Some pte_of_def obind_def split: option.splits)
-apply fastforce
-apply fastforce
-apply fastforce
-apply clarsimp
-apply clarsimp
-
-apply (prop_tac "level_of_slot asida vrefa p s = level'")
-apply (erule level_of_slot_vs_lookup_slot)
-apply fastforce+
-apply (simp only:)
-apply (thin_tac "level_of_slot _ _ _ _ = _")
-
-apply (clarsimp simp: vs_lookup_slot_def split: if_splits)
-  by (metis vs_lookup_slot_table vs_lookup_slot_unique_level)
-
-
-definition level_of_table :: "obj_ref \<Rightarrow> 'z::state_ext state \<Rightarrow> vm_level"
+definition level_of_table :: "obj_ref \<Rightarrow> 'z :: state_ext state \<Rightarrow> vm_level"
   where
   "level_of_table p s \<equiv>
-     GREATEST level. \<exists>asid vref. vref \<in> user_region \<and> vs_lookup_table level asid vref s = Some (level, p)"
+     GREATEST lvl. \<exists>asid vref. vref \<in> user_region \<and> vs_lookup_table lvl asid vref s = Some (lvl, p)"
 
 lemma level_of_table_vs_lookup_table:
   "\<lbrakk> vs_lookup_table level asid vref s = Some (level, p);
      ptes_of s p = Some pte; level \<le> max_pt_level; vref \<in> user_region; invs s \<rbrakk>
      \<Longrightarrow> level_of_table p s = level"
-apply (subst level_of_table_def)
-apply (rule Greatest_equality)
-apply fastforce
-apply clarsimp
-thm vs_lookup_slot_no_asid vs_lookup_slot_unique_level
-    apply (case_tac "y = asid_pool_level")
-apply clarsimp
-apply (drule vs_lookup_table_no_asid)
-apply simp
-apply clarsimp+
-
-apply (drule (1) vs_lookup_table_unique_level)
-apply fastforce+
-done
-
+  apply (subst level_of_table_def)
+  apply (rule Greatest_equality, fastforce)
+  apply (case_tac "y = asid_pool_level")
+   apply (fastforce dest: vs_lookup_table_no_asid)
+  apply (fastforce dest: vs_lookup_table_unique_level)
+  done
 
 lemma state_vrefs_store_NonPageTablePTE':
-  "\<lbrakk> invs s; is_aligned p pte_bits; \<forall>level asid vref. vref \<in> user_region \<longrightarrow> vs_lookup_slot level asid vref s \<noteq> Some (level, p);
-     \<not> is_PageTablePTE pte;
-     kheap s (table_base p) = Some (ArchObj (PageTable pt)) \<rbrakk>
+  "\<lbrakk> invs s; is_aligned p pte_bits; \<not> is_PageTablePTE pte;
+     kheap s (table_base p) = Some (ArchObj (PageTable pt));
+     \<forall>level asid vref. vref \<in> user_region \<longrightarrow> vs_lookup_slot level asid vref s \<noteq> Some (level, p) \<rbrakk>
      \<Longrightarrow> state_vrefs (s\<lparr>kheap := \<lambda>a. if a = table_base p
-                                     then Some (ArchObj (PageTable (\<lambda>a. if a = table_index p then pte else pt a)))
+                                     then Some (ArchObj (PageTable (\<lambda>a. if a = table_index p
+                                                                        then pte
+                                                                        else pt a)))
                                      else kheap s a\<rparr>) =
          (\<lambda>x. if x = table_base p \<and> (\<exists>level. \<exists>\<rhd> (level, table_base p) s)
-                    then vs_refs_aux (level_of_table (table_base p) s) (PageTable (\<lambda>a. if a = table_index p then pte else pt a))
+              then vs_refs_aux (level_of_table (table_base p) s) (PageTable (\<lambda>a. if a = table_index p
+                                                                                 then pte
+                                                                                 else pt a))
               else state_vrefs s x)"
   apply (rule all_ext)
   apply safe
-
-
-(* first thing *)
    apply (subst (asm) state_vrefs_def opt_map_def)+
    apply (clarsimp split: option.splits split del: if_split)
    apply (clarsimp split: if_split_asm option.splits split del: if_split)
-
-(* x = table_base p *)
     apply (subst (asm) vs_lookup_non_PageTablePTE[where s=s and p=p and pte=pte])
-           apply (clarsimp simp: ptes_of_Some pts_of_Some aobjs_of_Some)
-          apply (rule all_ext)
-          apply (clarsimp simp: opt_map_def pte_of_def obind_def)
-          apply (fastforce dest: pte_ptr_eq)
-         apply simp
-        apply (fastforce simp: opt_map_def)
-       apply (fastforce simp: opt_map_def)
-      apply fastforce+
-    (* done *)
-
+           apply (fastforce dest: pte_ptr_eq
+                            simp: ptes_of_Some pts_of_Some aobjs_of_Some
+                                  opt_map_def pte_of_def obind_def)+
     apply (clarsimp split: if_splits)
-apply safe
-
+    apply (drule vs_lookup_level)
+    apply (rule conjI; clarsimp)
     apply (case_tac "level = asid_pool_level")
-         apply (fastforce dest: vs_lookup_table_no_asid
-                          simp: ptes_of_Some pts_of_Some aobjs_of_Some pte_of_def obind_def
-                         split: option.splits)
+     apply (fastforce dest: vs_lookup_table_no_asid simp: ptes_of_Some pts_of_Some aobjs_of_Some)
     apply (case_tac "lvl = asid_pool_level")
-      apply (drule vs_lookup_level)
-      apply (fastforce dest: vs_lookup_table_no_asid
-                       simp: ptes_of_Some pts_of_Some aobjs_of_Some pte_of_def obind_def
-                      split: option.splits)
+     apply (fastforce dest: vs_lookup_table_no_asid simp: ptes_of_Some pts_of_Some aobjs_of_Some)
+    apply (subst level_of_table_vs_lookup_table; fastforce simp: ptes_of_Some pts_of_Some aobjs_of_Some)
+   apply (subst (asm) vs_lookup_non_PageTablePTE[where s=s and p=p and pte=pte])
+          apply (fastforce dest: pte_ptr_eq
+                           simp: ptes_of_Some pts_of_Some aobjs_of_Some
+                                 opt_map_def pte_of_def obind_def)+
+   apply (fastforce simp: state_vrefs_def aobjs_of_Some)
+  apply (clarsimp split: if_splits)
+   apply (case_tac "level = asid_pool_level")
+    apply (fastforce dest: vs_lookup_table_no_asid simp: ptes_of_Some pts_of_Some aobjs_of_Some)
+   apply (subst (asm) level_of_table_vs_lookup_table)
+        apply (fastforce simp: ptes_of_Some pts_of_Some aobjs_of_Some)+
+   apply (rule state_vrefsD)
+      apply (subst vs_lookup_non_PageTablePTE[where s=s and p=p and pte=pte ])
+             apply ((fastforce dest: pte_ptr_eq
+                               simp: ptes_of_Some pts_of_Some aobjs_of_Some
+                                     opt_map_def pte_of_def obind_def)+)[7]
+      apply auto[1]
+     apply (fastforce simp: aobjs_of_Some opt_map_def)
+    apply clarsimp
+   apply clarsimp
+  apply (case_tac "x = table_base p")
+   apply (fastforce dest: vs_lookup_level simp: state_vrefs_def)
+  apply (subst (asm) state_vrefs_def, clarsimp)
+  apply (rule state_vrefsD)
+     apply (subst vs_lookup_non_PageTablePTE[where s=s and p=p and pte=pte ])
+            apply ((fastforce dest: pte_ptr_eq
+                              simp: ptes_of_Some pts_of_Some aobjs_of_Some
+                                    opt_map_def pte_of_def obind_def)+)[7]
+     apply auto[1]
+    apply (fastforce simp: aobjs_of_Some opt_map_def split: option.splits)
+   apply clarsimp
+  apply clarsimp
+  done
 
-
-apply (prop_tac "level_of_table (table_base p) s = level")
-
-apply (erule level_of_table_vs_lookup_table)
-apply (fastforce simp: ptes_of_Some pte_of_def obind_def pts_of_Some aobjs_of_Some split: option.splits)
-apply fastforce+
-
-apply clarsimp
-apply (drule vs_lookup_level)
-apply (drule (1) vs_lookup_table_unique_level)
-apply fastforce
-apply fastforce
-apply fastforce
-apply fastforce
-apply fastforce
-apply fastforce
-apply fastforce
-apply (fastforce dest: vs_lookup_level)
-
-
-(* x = table_base p *)
-    apply (subst (asm) vs_lookup_non_PageTablePTE[where s=s and p=p and pte=pte])
-           apply (clarsimp simp: ptes_of_Some pts_of_Some aobjs_of_Some)
-          apply (rule all_ext)
-          apply (clarsimp simp: opt_map_def pte_of_def obind_def)
-          apply (fastforce dest: pte_ptr_eq)
-         apply simp
-        apply (fastforce simp: opt_map_def)
-       apply (fastforce simp: opt_map_def)
-      apply fastforce+
-    (* done *)
-    apply (clarsimp split: if_splits)
-apply (clarsimp simp: state_vrefs_def)
-apply (fastforce simp: aobjs_of_Some)
-
-
-
-apply (clarsimp split: if_splits)
-
-
-    apply (case_tac "level = asid_pool_level")
-         apply (fastforce dest: vs_lookup_table_no_asid
-                          simp: ptes_of_Some pts_of_Some aobjs_of_Some pte_of_def obind_def
-                         split: option.splits)
-
-apply (prop_tac "level_of_table (table_base p) s = level")
-apply (erule level_of_table_vs_lookup_table)
-apply (fastforce simp: ptes_of_Some pte_of_def obind_def pts_of_Some aobjs_of_Some split: option.splits)
-apply fastforce+
-
-apply (simp only:)
-apply (thin_tac "level_of_table _ _ = _")
-
-  apply (clarsimp simp: state_vrefs_def opt_map_def)
-
-apply (intro exI conjI)
-apply (rule refl)
-apply (subst vs_lookup_non_PageTablePTE[where s=s and p=p and pte=pte ])
-apply (clarsimp simp: ptes_of_Some pts_of_Some aobjs_of_Some)
- apply (rule all_ext)
-        apply (clarsimp simp: opt_map_def pte_of_def obind_def)
-        apply (fastforce dest: pte_ptr_eq)
-       apply simp
-      apply (fastforce simp: opt_map_def)
-     apply (fastforce simp: opt_map_def)
-    apply fastforce
-    apply fastforce
-defer
-apply fastforce
-apply fastforce
-apply fastforce
-defer
-apply (clarsimp split: if_splits)
-apply auto[1]
-
-apply (case_tac "x = table_base p"; clarsimp)
-apply (clarsimp simp: state_vrefs_def)
-apply (fastforce dest: vs_lookup_level)
-
-  apply (clarsimp simp: state_vrefs_def opt_map_def)
-
-apply (intro exI conjI)
-apply (rule refl)
-apply (subst vs_lookup_non_PageTablePTE[where s=s and p=p and pte=pte ])
-apply (clarsimp simp: ptes_of_Some pts_of_Some aobjs_of_Some)
- apply (rule all_ext)
-        apply (clarsimp simp: opt_map_def pte_of_def obind_def)
-        apply (fastforce dest: pte_ptr_eq)
-       apply simp
-      apply (fastforce simp: opt_map_def)
-     apply (fastforce simp: opt_map_def)
-    apply fastforce
-    apply fastforce
-defer
-apply fastforce
-apply fastforce
-apply fastforce
-defer
-apply (clarsimp split: if_splits)
-apply auto[1]
-done
-
-
-
-lemma state_vrefs_store_NonPageTablePTE_wp':
-"\<lbrace>\<lambda>s. invs s \<and> \<not> is_PageTablePTE pte \<and>
-
-(\<forall>pt. ako_at (PageTable pt) (table_base p) s \<longrightarrow> is_aligned p pte_bits \<longrightarrow>
- (if \<exists>level asid vref. vs_lookup_slot level asid vref s = Some (level, p) \<and> vref \<in> user_region
-  then (\<exists>level asid vref. vs_lookup_slot level asid vref s = Some (level, p) \<and> vref \<in> user_region \<and>
-                          P (\<lambda>x. (if \<exists>level' vref'. vref' \<in> user_region \<and> vref_for_level vref' (level + 1) = vref_for_level vref (level + 1) \<and>
-                                                    p = pt_slot_offset level (table_base p) vref' \<and>
-                                                    pt_walk level level' (table_base p) vref' (ptes_of s) = Some (level',x)
-                                  then (if x = table_base p
-                                        then vs_refs_aux level (PageTable (\<lambda>a. if a = table_index p then pte else pt a))
-                                        else {})
-                                  else state_vrefs s x)))
-else P (\<lambda>x. (if x = table_base p \<and> (\<exists>level. \<exists>\<rhd> (level, table_base p) s)
-                    then vs_refs_aux (level_of_table (table_base p) s) (PageTable (\<lambda>a. if a = table_index p then pte else pt a))
-              else state_vrefs s x))))
-\<rbrace> store_pte p pte \<lbrace>\<lambda>_ s. P (state_vrefs s)\<rbrace>"
-unfolding store_pte_def set_pt_def
-apply (wpsimp wp: set_object_wp)
-apply (case_tac "\<exists>level asid vref.
-                           vs_lookup_slot level asid vref s = Some (level, p) \<and> vref \<in> user_region")
-apply (erule_tac x=pt in allE)
-apply clarsimp
-apply (clarsimp simp: fun_upd_def)
-apply (subst state_vrefs_store_NonPageTablePTE)
-apply fastforce+
-apply (clarsimp simp: obj_at_def)
-apply (case_tac "level = asid_pool_level")
-     apply (fastforce dest: vs_lookup_slot_no_asid
-                      simp: ptes_of_Some pts_of_Some aobjs_of_Some pte_of_def obind_def obj_at_def
-                      split: option.splits)
-
-apply (case_tac "levela = asid_pool_level")
-     apply (fastforce dest: vs_lookup_slot_no_asid
-                      simp: ptes_of_Some pts_of_Some aobjs_of_Some pte_of_def obind_def obj_at_def
-                      split: option.splits)
-apply (drule (1) vs_lookup_slot_unique_level)
-apply fastforce+
-apply clarsimp
-apply (prop_tac "vref_for_level vrefa (level+1) = vref_for_level vref (level+1)")
-  apply (metis (mono_tags, hide_lams) vs_lookup_slot_table_base vs_lookup_slot_vref_for_level_eq vs_lookup_table_unique_level)
-apply clarsimp
-
-apply clarsimp
-apply (erule_tac x=pt in allE)
-apply (clarsimp simp: fun_upd_def)
-apply (subst state_vrefs_store_NonPageTablePTE')
-apply fastforce+
-apply (clarsimp simp: obj_at_def)
-apply clarsimp
-done
-
-
+(* FIXME AC: make this less ugly *)
+lemma state_vrefs_store_NonPageTablePTE_wp:
+  "\<lbrace>\<lambda>s. invs s \<and> \<not> is_PageTablePTE pte \<and>
+        (\<forall>pt. ako_at (PageTable pt) (table_base p) s \<and> is_aligned p pte_bits \<longrightarrow>
+              (if \<exists>level asid vref. vs_lookup_slot level asid vref s = Some (level, p) \<and> vref \<in> user_region
+               then (\<exists>level asid vref. vs_lookup_slot level asid vref s = Some (level, p) \<and> vref \<in> user_region \<and>
+                                       P (\<lambda>x. (if \<exists>level' vref'. vref_for_level vref' (level + 1) = vref_for_level vref (level + 1) \<and>
+                                                                 vref' \<in> user_region \<and> p = pt_slot_offset level (table_base p) vref' \<and>
+                                                                 pt_walk level level' (table_base p) vref' (ptes_of s) = Some (level', x)
+                                               then (if x = table_base p
+                                                     then vs_refs_aux level (PageTable (\<lambda>a. if a = table_index p then pte else pt a))
+                                                     else {})
+                                               else state_vrefs s x)))
+               else P (\<lambda>x. (if x = table_base p \<and> (\<exists>level. \<exists>\<rhd> (level, table_base p) s)
+                            then vs_refs_aux (level_of_table (table_base p) s) (PageTable (\<lambda>a. if a = table_index p then pte else pt a))
+                            else state_vrefs s x))))\<rbrace>
+   store_pte p pte
+   \<lbrace>\<lambda>_ s. P (state_vrefs s)\<rbrace>"
+  unfolding store_pte_def set_pt_def
+  apply (wpsimp wp: set_object_wp)
+  apply (case_tac "\<exists>level asid vref. vs_lookup_slot level asid vref s = Some (level, p) \<and>
+                                     vref \<in> user_region")
+   apply (erule_tac x=pt in allE)
+   apply (clarsimp simp: fun_upd_def)
+   apply (subst state_vrefs_store_NonPageTablePTE)
+         apply fastforce+
+    apply (clarsimp simp: obj_at_def)
+   apply (case_tac "level = asid_pool_level")
+    apply (fastforce dest: vs_lookup_slot_no_asid
+                     simp: ptes_of_Some pts_of_Some aobjs_of_Some obj_at_def)
+   apply (case_tac "levela = asid_pool_level")
+    apply (fastforce dest: vs_lookup_slot_no_asid
+                     simp: ptes_of_Some pts_of_Some aobjs_of_Some obj_at_def)
+   apply (drule (1) vs_lookup_slot_unique_level)
+         apply fastforce+
+   apply clarsimp
+   apply (frule_tac level'="level+1" in vref_for_level_eq_mono)
+    apply (fastforce intro: vm_level_less_le_1)
+   apply clarsimp
+  apply (erule_tac x=pt in allE)
+  apply (clarsimp simp: fun_upd_def)
+  apply (subst state_vrefs_store_NonPageTablePTE'; fastforce simp: obj_at_def)
+  done
 
 definition authorised_page_table_inv :: "'a PAS \<Rightarrow> page_table_invocation \<Rightarrow> bool" where
   "authorised_page_table_inv aag pti \<equiv>
@@ -1100,33 +600,32 @@ definition authorised_page_table_inv :: "'a PAS \<Rightarrow> page_table_invocat
                  is_subject aag (fst cslot_ptr) \<and> is_subject aag (obj_ref && ~~ mask pt_bits) \<and>
                  pas_cap_cur_auth aag (ArchObjectCap cap)
              | PageTableUnmap cap cslot_ptr \<Rightarrow>
-                 is_subject aag (fst cslot_ptr) \<and> aag_cap_auth aag (pasSubject aag) (ArchObjectCap cap)  \<and>
+                 is_subject aag (fst cslot_ptr) \<and>
+                 aag_cap_auth aag (pasSubject aag) (ArchObjectCap cap) \<and>
                  (\<forall>p asid vspace_ref. cap = PageTableCap p (Some (asid, vspace_ref))
                                       \<longrightarrow> is_subject_asid aag asid \<and>
-                                          (\<forall>x \<in> set [p , p + 2 ^ pte_bits .e. p + 2 ^ pt_bits - 1].
-                                                   is_subject aag (x && ~~ mask pt_bits)))"
+                                          (\<forall>x \<in> set [p, p + 2 ^ pte_bits .e. p + 2 ^ pt_bits - 1].
+                                                             is_subject aag (x && ~~ mask pt_bits)))"
 
 lemma store_pte_thread_states[wp]:
   "store_pte p pte \<lbrace>\<lambda>s. P (thread_states s)\<rbrace>"
-unfolding store_pte_def set_pt_def
-apply (wpsimp wp: set_object_wp)
+  unfolding store_pte_def set_pt_def
+  apply (wpsimp wp: set_object_wp)
   apply (clarsimp simp: get_tcb_def thread_states_def tcb_states_of_state_def obj_at_def
                  elim!: rsubst[where P=P, OF _ ext])
-done
+  done
 
 lemma store_pte_thread_bound_ntfns[wp]:
   "store_pte p pte \<lbrace>\<lambda>s. P (thread_bound_ntfns s)\<rbrace>"
-unfolding store_pte_def set_pt_def
-apply (wpsimp wp: set_object_wp)
+  unfolding store_pte_def set_pt_def
+  apply (wpsimp wp: set_object_wp)
   apply (clarsimp simp: get_tcb_def thread_bound_ntfns_def  obj_at_def
                  elim!: rsubst[where P=P, OF _ ext])
-done
+  done
 
 lemma store_pte_domains_of_state[wp]:
   "store_pte p pte \<lbrace>\<lambda>s. P (domains_of_state s)\<rbrace>"
-unfolding store_pte_def set_pt_def
-by (wpsimp wp: set_object_wp)
-
+  unfolding store_pte_def set_pt_def by (wpsimp wp: set_object_wp)
 
 lemma mapM_x_store_pte_caps_of_state[wp]:
   "mapM_x (swp store_pte InvalidPTE) slots \<lbrace>\<lambda>s. P (asid_table s)\<rbrace>"
@@ -1148,488 +647,103 @@ lemma state_asids_to_policy_vrefs_subseteq:
   apply (erule state_asids_to_policy_aux.cases; fastforce intro: state_asids_to_policy_aux.intros)
   done
 
-
 lemma store_pte_state_objs_in_policy:
-  "\<lbrace>(\<lambda>s. state_objs_in_policy aag s) and invs
-and (\<lambda>s. (\<exists>slot ref. caps_of_state s slot = Some (ArchObjectCap (PageTableCap (table_base p) ref)))
-\<and>  ((\<exists>asid. vspace_for_asid asid s = Some (table_base p)) \<longrightarrow> table_index p \<notin> kernel_mapping_slots) \<and>
-                table_base p \<notin> global_refs s
-)\<rbrace>
- store_pte p InvalidPTE
-\<lbrace>\<lambda>_ s. state_objs_in_policy aag s\<rbrace>"
-
+  "\<lbrace>\<lambda>s. state_objs_in_policy aag s \<and> invs s \<and> table_base p \<notin> global_refs s \<and>
+        ((\<exists>a. vspace_for_asid a s = Some (table_base p)) \<longrightarrow> table_index p \<notin> kernel_mapping_slots)\<rbrace>
+   store_pte p InvalidPTE
+   \<lbrace>\<lambda>_ s. state_objs_in_policy aag s\<rbrace>"
   apply (rule hoare_weaken_pre)
    apply (clarsimp simp: state_objs_to_policy_def pred_conj_def)
    apply wps
-   apply (rule state_vrefs_store_NonPageTablePTE_wp')
+   apply (rule state_vrefs_store_NonPageTablePTE_wp)
   apply clarsimp
-  apply (rule conjI)
-   apply clarsimp
-   apply (rule exI)+
-   apply (rule conjI, assumption)
-   apply clarsimp
-
+  apply (rule conjI; clarsimp)
+   apply (intro exI conjI)
+     apply assumption
+    apply clarsimp
    apply (clarsimp simp: state_objs_to_policy_def)
    apply (erule subsetD)
    apply (clarsimp simp: auth_graph_map_def)
    apply (rule exI, rule conjI, rule refl)+
-   apply (erule state_bits_to_policy_vrefs_subseteq)
-       apply clarsimp
-       apply clarsimp
-       apply clarsimp
-       apply clarsimp
-
-   apply clarsimp
-   apply (clarsimp simp: state_vrefs_def)
-   apply (rule exI)
-   apply (rule conjI)
-    apply (rule_tac x=level in exI)
-    apply (rule_tac x="PageTable pt" in exI)
-    apply (rule conjI, rule refl)
-
-    apply (case_tac "level = asid_pool_level")
-     apply (fastforce dest: vs_lookup_slot_no_asid
-                      simp: ptes_of_Some pts_of_Some aobjs_of_Some pte_of_def obind_def obj_at_def
-                      split: option.splits)
-
-
-    apply (subst (asm) vs_lookup_slot_table_unfold)
-       apply fastforce+
-    apply (fastforce simp: aobjs_of_Some obj_at_def)
-   apply (clarsimp simp: vs_refs_aux_def
-   graph_of_def)
-   apply (clarsimp split: if_splits)
-    apply (clarsimp simp: pte_ref2_def)
-   apply fastforce
-
+   apply (erule state_bits_to_policy_vrefs_subseteq; clarsimp)
+   apply (case_tac "level = asid_pool_level")
+    apply (fastforce dest: vs_lookup_slot_no_asid
+                     simp: ptes_of_Some pts_of_Some aobjs_of_Some obj_at_def)
+   apply (subst (asm) vs_lookup_slot_table_unfold; clarsimp)
+   apply (erule state_vrefsD)
+     apply (fastforce simp: aobjs_of_Some obj_at_def)
+    apply clarsimp
+   apply (fastforce simp: vs_refs_aux_def graph_of_def pte_ref2_def split: if_splits)
   apply (clarsimp simp: state_objs_to_policy_def)
   apply (erule subsetD)
   apply (clarsimp simp: auth_graph_map_def)
   apply (rule exI, rule conjI, rule refl)+
-  apply (erule state_bits_to_policy_vrefs_subseteq)
-       apply clarsimp
-       apply clarsimp
-       apply clarsimp
-       apply clarsimp
-  apply clarsimp
-  apply (clarsimp simp: state_vrefs_def)
-  apply (rule exI)
-  apply (rule conjI)
-   apply (rule_tac x=level in exI)
-   apply (rule_tac x="PageTable pt" in exI)
-   apply (rule conjI, rule refl)
-
-   apply (fastforce simp: aobjs_of_Some obj_at_def)
-
+  apply (erule state_bits_to_policy_vrefs_subseteq; clarsimp)
   apply (case_tac "level = asid_pool_level")
    apply (fastforce dest: vs_lookup_table_no_asid
-                    simp: ptes_of_Some pts_of_Some aobjs_of_Some pte_of_def obind_def obj_at_def
-                    split: option.splits)
-  apply (drule level_of_table_vs_lookup_table)
+                    simp: ptes_of_Some pts_of_Some aobjs_of_Some obj_at_def)
+  apply (frule level_of_table_vs_lookup_table)
       apply (fastforce dest: vs_lookup_slot_no_asid
-                       simp: ptes_of_Some pts_of_Some aobjs_of_Some pte_of_def obind_def obj_at_def
-                       split: option.splits)+
-  apply (simp only:)
-  apply (thin_tac "level_of_table _ _ = _")
-  apply (clarsimp simp: vs_refs_aux_def
-  graph_of_def)
-  apply (clarsimp split: if_splits)
-   apply (clarsimp simp: pte_ref2_def)
-  apply fastforce
-
-  done
-
-
-
-(*
-lemma store_pte_state_objs_in_policy:
-  "\<forall>X Y. (\<forall>x. X x \<subseteq> Y x) \<longrightarrow> P Y \<longrightarrow> P X \<Longrightarrow>
-
-\<lbrace>\<lambda>s. P (state_vrefs s) \<and> invs s \<and> \<not> is_PageTablePTE pte \<and>
-(\<exists>slot ref. caps_of_state s slot = Some (ArchObjectCap (PageTableCap (table_base p) ref)))
-\<and>  ((\<exists>asid. vspace_for_asid asid s = Some (table_base p)) \<longrightarrow> table_index p \<notin> kernel_mapping_slots) \<and>
-                table_base p \<notin> global_refs s\<rbrace>
- store_pte p pte
-\<lbrace>\<lambda>_ s. P (state_vrefs s)\<rbrace>"
-  apply (rule hoare_weaken_pre)
-   apply (rule state_vrefs_store_NonPageTablePTE_wp')
-  apply clarsimp
-  apply (rule conjI)
-   apply clarsimp
-   apply (rule exI)+
-   apply (rule conjI, assumption)
-   apply clarsimp
-
-apply (erule_tac x="(\<lambda>a. if \<exists>level' vref'.
-                         vref' \<in> user_region \<and>
-                         vref_for_level vref' (level + 1) = vref_for_level vref (level + 1) \<and>
-                         p = pt_slot_offset level (table_base p) vref' \<and>
-                         pt_walk level level' (table_base p) vref' (ptes_of s) = Some (level', a)
-                   then if a = table_base p then vs_refs_aux level (PageTable (\<lambda>a. if a = table_index p then pte else pt a))
-                        else {}
-                   else state_vrefs s a)" in allE)
-apply (erule_tac x="state_vrefs s" in allE)
-
-apply (drule mp) back
-prefer 2
-apply clarsimp
-
-apply clarsimp
-
-
-   apply (clarsimp simp: state_vrefs_def)
-   apply (rule exI)
-   apply (rule conjI)
-    apply (rule_tac x=level in exI)
-    apply (rule_tac x="PageTable pt" in exI)
-    apply (rule conjI, rule refl)
-
-    apply (case_tac "level = asid_pool_level")
-     apply (fastforce dest: vs_lookup_slot_no_asid
-                      simp: ptes_of_Some pts_of_Some aobjs_of_Some pte_of_def obind_def obj_at_def
-                      split: option.splits)
-
-
-    apply (subst (asm) vs_lookup_slot_table_unfold)
-       apply fastforce+
+                       simp: ptes_of_Some pts_of_Some aobjs_of_Some obj_at_def)+
+  apply (erule state_vrefsD)
     apply (fastforce simp: aobjs_of_Some obj_at_def)
-
-apply (clarsimp simp: vs_refs_aux_def graph_of_def)
-apply (case_tac "ad = table_index p"; clarsimp)
-
-
-apply (case_tac
-
-   apply (clarsimp simp: vs_refs_aux_def
-   graph_of_def)
-   apply (clarsimp split: if_splits)
-    apply (clarsimp simp: pte_ref2_def)
-apply (case_tac pte; clarsimp)
-   apply fastforce
-
-apply clarsimp
-
-
-apply (erule_tac x="(\<lambda>a. if a = table_base p \<and> (\<exists>level. \<exists>\<rhd> (level, table_base p) s)
-                   then vs_refs_aux (level_of_table (table_base p) s)
-                         (PageTable (\<lambda>a. if a = table_index p then InvalidPTE else pt a))
-                   else state_vrefs s a)" in allE)
-apply (erule_tac x="state_vrefs s" in allE)
-
-apply (drule mp) back
-prefer 2
-apply clarsimp
-
-
-  apply (clarsimp simp: state_vrefs_def)
-  apply (rule exI)
-  apply (rule conjI)
-   apply (rule_tac x=level in exI)
-   apply (rule_tac x="PageTable pt" in exI)
-   apply (rule conjI, rule refl)
-
-   apply (fastforce simp: aobjs_of_Some obj_at_def)
-
-  apply (case_tac "level = asid_pool_level")
-   apply (fastforce dest: vs_lookup_table_no_asid
-                    simp: ptes_of_Some pts_of_Some aobjs_of_Some pte_of_def obind_def obj_at_def
-                    split: option.splits)
-  apply (drule level_of_table_vs_lookup_table)
-      apply (fastforce dest: vs_lookup_slot_no_asid
-                       simp: ptes_of_Some pts_of_Some aobjs_of_Some pte_of_def obind_def obj_at_def
-                       split: option.splits)+
-  apply (simp only:)
-  apply (thin_tac "level_of_table _ _ = _")
-  apply (clarsimp simp: vs_refs_aux_def
-  graph_of_def)
-  apply (clarsimp split: if_splits)
-   apply (clarsimp simp: pte_ref2_def)
-  apply fastforce
+   apply clarsimp
+  apply (fastforce simp: vs_refs_aux_def graph_of_def pte_ref2_def split: if_splits)
   done
-*)
-
-
-lemma store_pte_mapM_x_state_objs_in_policy:
- "\<lbrace>state_objs_in_policy aag and invs and
-   (\<lambda>s. \<forall>x \<in> set slots. table_base x \<notin> global_refs s \<and> (\<forall>asid. vspace_for_asid asid s \<noteq> Some (table_base x))
-)\<rbrace>
- mapM_x (swp store_pte InvalidPTE) slots
-\<lbrace>\<lambda>_. state_objs_in_policy aag\<rbrace>"
-apply (rule hoare_strengthen_post)
-apply (rule mapM_x_wp[where S="set slots"])
-
-apply (rule hoare_weaken_pre)
-apply (clarsimp simp: state_objs_to_policy_def pred_conj_def)
-apply (rule hoare_vcg_conj_lift)
-apply wps
-apply (rule state_vrefs_store_NonPageTablePTE_wp')
-   apply (wp store_pte_invs hoare_vcg_const_Ball_lift hoare_vcg_ex_lift hoare_vcg_all_lift)
-apply clarsimp
-   apply (clarsimp simp: wellformed_pte_def)
-apply (rule conjI)
-apply (thin_tac P for P)
-apply clarsimp
-apply (rule exI)+
-apply (rule conjI, assumption)
-apply clarsimp
-
-apply (clarsimp simp: state_objs_to_policy_def)
-apply (erule subsetD)
-apply (clarsimp simp: auth_graph_map_def)
-apply (rule exI, rule conjI, rule refl)+
-apply (erule state_bits_to_policy_vrefs_subseteq)
-       apply clarsimp
-       apply clarsimp
-       apply clarsimp
-       apply clarsimp
-apply clarsimp
-apply (clarsimp simp: state_vrefs_def)
-apply (rule exI)
-apply (rule conjI)
-apply (rule_tac x=level in exI)
-apply (rule_tac x="PageTable pt" in exI)
-apply (rule conjI, rule refl)
-
-apply (case_tac "level = asid_pool_level")
-     apply (fastforce dest: vs_lookup_slot_no_asid
-                      simp: ptes_of_Some pts_of_Some aobjs_of_Some pte_of_def obind_def obj_at_def
-                      split: option.splits)
-
-
-apply (subst (asm) vs_lookup_slot_table_unfold)
-apply fastforce+
-apply (fastforce simp: aobjs_of_Some obj_at_def)
-apply (clarsimp simp: vs_refs_aux_def
-graph_of_def)
-apply (clarsimp split: if_splits)
-apply (clarsimp simp: pte_ref2_def)
-apply fastforce
-
-apply (clarsimp simp: state_objs_to_policy_def)
-apply (erule subsetD)
-apply (clarsimp simp: auth_graph_map_def)
-apply (rule exI, rule conjI, rule refl)+
-apply (erule state_bits_to_policy_vrefs_subseteq)
-       apply clarsimp
-       apply clarsimp
-       apply clarsimp
-       apply clarsimp
-apply clarsimp
-apply (clarsimp simp: state_vrefs_def)
-apply (rule exI)
-apply (rule conjI)
-apply (rule_tac x=level in exI)
-apply (rule_tac x="PageTable pt" in exI)
-apply (rule conjI, rule refl)
-
-apply (fastforce simp: aobjs_of_Some obj_at_def)
-
-apply (case_tac "level = asid_pool_level")
-     apply (fastforce dest: vs_lookup_table_no_asid
-                      simp: ptes_of_Some pts_of_Some aobjs_of_Some pte_of_def obind_def obj_at_def
-                      split: option.splits)
-apply (drule level_of_table_vs_lookup_table)
-     apply (fastforce dest: vs_lookup_slot_no_asid
-                      simp: ptes_of_Some pts_of_Some aobjs_of_Some pte_of_def obind_def obj_at_def
-                      split: option.splits)+
-apply (simp only:)
-apply (thin_tac "level_of_table _ _ = _")
-apply (clarsimp simp: vs_refs_aux_def
-graph_of_def)
-apply (clarsimp split: if_splits)
-apply (clarsimp simp: pte_ref2_def)
-apply fastforce
-
-apply clarsimp
-
-apply clarsimp
-done
 
 lemma store_pte_state_asids_to_policy:
-  "\<lbrace>(\<lambda>s. state_asids_to_policy aag s \<subseteq> pasPolicy aag) and invs
-and (\<lambda>s. (\<exists>slot ref. caps_of_state s slot = Some (ArchObjectCap (PageTableCap (table_base p) ref)))
-\<and>  ((\<exists>asid. vspace_for_asid asid s = Some (table_base p)) \<longrightarrow> table_index p \<notin> kernel_mapping_slots) \<and>
-                table_base p \<notin> global_refs s
-)\<rbrace>
- store_pte p InvalidPTE
-\<lbrace>\<lambda>_ s. state_asids_to_policy aag s \<subseteq> pasPolicy aag\<rbrace>"
-apply (rule hoare_weaken_pre)
-apply (clarsimp simp: state_objs_to_policy_def pred_conj_def)
-apply wps
-apply (rule state_vrefs_store_NonPageTablePTE_wp')
-   apply (wpsimp wp: store_pte_invs hoare_vcg_const_Ball_lift hoare_vcg_ex_lift hoare_vcg_all_lift hoare_vcg_imp_lift')
-
-apply (rule conjI)
-apply clarsimp
-
-apply (rule exI)+
-apply (rule conjI, assumption)
-apply clarsimp
-
-apply (erule subsetD)
-apply (erule state_asids_to_policy_vrefs_subseteq)
-apply clarsimp
-apply clarsimp
-apply (clarsimp simp: state_vrefs_def)
-apply (rule exI)
-apply (rule conjI)
-apply (rule_tac x=level in exI)
-apply (rule_tac x="PageTable pt" in exI)
-apply (rule conjI, rule refl)
-
-apply (case_tac "level = asid_pool_level")
-     apply (fastforce dest: vs_lookup_slot_no_asid
-                      simp: ptes_of_Some pts_of_Some aobjs_of_Some pte_of_def obind_def obj_at_def
-                      split: option.splits)
-
-
-apply (subst (asm) vs_lookup_slot_table_unfold)
-apply fastforce+
-apply (fastforce simp: aobjs_of_Some obj_at_def)
-apply (clarsimp simp: vs_refs_aux_def
-graph_of_def)
-apply (clarsimp split: if_splits)
-apply (clarsimp simp: pte_ref2_def)
-apply fastforce
-
-apply clarsimp
-
-apply (clarsimp)
-apply (erule subsetD)
-apply (erule state_asids_to_policy_vrefs_subseteq)
-apply clarsimp
-
-apply clarsimp
-apply (clarsimp simp: state_vrefs_def)
-apply (rule exI)
-apply (rule conjI)
-apply (rule_tac x=level in exI)
-apply (rule_tac x="PageTable pt" in exI)
-apply (rule conjI, rule refl)
-
-apply (fastforce simp: aobjs_of_Some obj_at_def)
-
-apply (case_tac "level = asid_pool_level")
-     apply (fastforce dest: vs_lookup_table_no_asid
-                      simp: ptes_of_Some pts_of_Some aobjs_of_Some pte_of_def obind_def obj_at_def
-                      split: option.splits)
-apply (drule level_of_table_vs_lookup_table)
-     apply (fastforce dest: vs_lookup_slot_no_asid
-                      simp: ptes_of_Some pts_of_Some aobjs_of_Some pte_of_def obind_def obj_at_def
-                      split: option.splits)+
-apply (simp only:)
-apply (thin_tac "level_of_table _ _ = _")
-apply (clarsimp simp: vs_refs_aux_def
-graph_of_def)
-apply (clarsimp split: if_splits)
-apply (clarsimp simp: pte_ref2_def)
-apply fastforce
-
-apply clarsimp
-done
-
-
-lemma store_pte_mapM_x_state_asids_to_policy:
- "\<lbrace>(\<lambda>s. state_asids_to_policy aag s \<subseteq> pasPolicy aag) and invs
-and (\<lambda>s. \<forall>x \<in> set slots. table_base x \<notin> global_refs s \<and> (\<forall>asid. vspace_for_asid asid s \<noteq> Some (table_base x)))\<rbrace>
- mapM_x (swp store_pte InvalidPTE) slots
-\<lbrace>\<lambda>_ s. state_asids_to_policy aag s \<subseteq> pasPolicy aag\<rbrace>"
-apply (rule hoare_strengthen_post)
-apply (rule mapM_x_wp[where S="set slots"])
-
-apply (rule hoare_weaken_pre)
-apply (clarsimp simp: state_objs_to_policy_def pred_conj_def)
-apply (rule hoare_vcg_conj_lift)
-apply wps
-apply (rule state_vrefs_store_NonPageTablePTE_wp')
-   apply (wpsimp wp: store_pte_invs hoare_vcg_const_Ball_lift hoare_vcg_ex_lift hoare_vcg_all_lift hoare_vcg_imp_lift')
-apply clarsimp
-   apply (clarsimp simp: wellformed_pte_def)
-apply (rule conjI)
-apply (thin_tac P for P)
-apply clarsimp
-
-apply (rule exI)+
-apply (rule conjI, assumption)
-apply clarsimp
-
-apply (erule subsetD)
-apply (erule state_asids_to_policy_vrefs_subseteq)
-apply clarsimp
-apply (clarsimp simp: state_vrefs_def)
-apply (rule exI)
-apply (rule conjI)
-apply (rule_tac x=level in exI)
-apply (rule_tac x="PageTable pt" in exI)
-apply (rule conjI, rule refl)
-
-apply (case_tac "level = asid_pool_level")
-     apply (fastforce dest: vs_lookup_slot_no_asid
-                      simp: ptes_of_Some pts_of_Some aobjs_of_Some pte_of_def obind_def obj_at_def
-                      split: option.splits)
-
-
-apply (subst (asm) vs_lookup_slot_table_unfold)
-apply fastforce+
-apply (fastforce simp: aobjs_of_Some obj_at_def)
-apply (clarsimp simp: vs_refs_aux_def
-graph_of_def)
-apply (clarsimp split: if_splits)
-apply (clarsimp simp: pte_ref2_def)
-apply fastforce
-apply clarsimp
-
-apply (clarsimp)
-apply (erule subsetD)
-apply (erule state_asids_to_policy_vrefs_subseteq)
-apply clarsimp
-apply (clarsimp simp: state_vrefs_def)
-apply (rule exI)
-apply (rule conjI)
-apply (rule_tac x=level in exI)
-apply (rule_tac x="PageTable pt" in exI)
-apply (rule conjI, rule refl)
-
-apply (fastforce simp: aobjs_of_Some obj_at_def)
-
-apply (case_tac "level = asid_pool_level")
-     apply (fastforce dest: vs_lookup_table_no_asid
-                      simp: ptes_of_Some pts_of_Some aobjs_of_Some pte_of_def obind_def obj_at_def
-                      split: option.splits)
-apply (drule level_of_table_vs_lookup_table)
-     apply (fastforce dest: vs_lookup_slot_no_asid
-                      simp: ptes_of_Some pts_of_Some aobjs_of_Some pte_of_def obind_def obj_at_def
-                      split: option.splits)+
-apply (simp only:)
-apply (thin_tac "level_of_table _ _ = _")
-apply (clarsimp simp: vs_refs_aux_def
-graph_of_def)
-apply (clarsimp split: if_splits)
-apply (clarsimp simp: pte_ref2_def)
-apply fastforce
-
-apply clarsimp
-apply clarsimp
-apply clarsimp
-done
-
-
-lemma mapM_x_store_pte_cdt[wp]:
-  "mapM_x (swp store_pte InvalidPTE) slots \<lbrace>\<lambda>s. P (cdt s)\<rbrace>"
-  by (wpsimp wp: mapM_x_wp')
+  "\<lbrace>\<lambda>s. state_asids_to_policy aag s \<subseteq> pasPolicy aag \<and> invs s \<and> table_base p \<notin> global_refs s \<and>
+        ((\<exists>a. vspace_for_asid a s = Some (table_base p)) \<longrightarrow> table_index p \<notin> kernel_mapping_slots)\<rbrace>
+   store_pte p InvalidPTE
+   \<lbrace>\<lambda>_ s. state_asids_to_policy aag s \<subseteq> pasPolicy aag\<rbrace>"
+  apply (rule hoare_weaken_pre)
+   apply (clarsimp simp: state_objs_to_policy_def pred_conj_def)
+   apply wps
+   apply (rule state_vrefs_store_NonPageTablePTE_wp)
+  apply clarsimp
+  apply (rule conjI; clarsimp)
+   apply (intro exI conjI)
+     apply assumption
+    apply clarsimp
+   apply clarsimp
+   apply (erule subsetD)
+   apply (erule state_asids_to_policy_vrefs_subseteq; clarsimp)
+   apply (case_tac "level = asid_pool_level")
+    apply (fastforce dest: vs_lookup_slot_no_asid
+                     simp: ptes_of_Some pts_of_Some aobjs_of_Some obj_at_def)
+   apply (subst (asm) vs_lookup_slot_table_unfold; clarsimp)
+   apply (erule state_vrefsD)
+     apply (fastforce simp: aobjs_of_Some obj_at_def)
+    apply clarsimp
+   apply (fastforce simp: vs_refs_aux_def graph_of_def pte_ref2_def split: if_splits)
+  apply (erule subsetD)
+  apply (erule state_asids_to_policy_vrefs_subseteq; clarsimp)
+  apply (case_tac "level = asid_pool_level")
+   apply (fastforce dest: vs_lookup_table_no_asid
+                    simp: ptes_of_Some pts_of_Some aobjs_of_Some obj_at_def)
+  apply (frule level_of_table_vs_lookup_table)
+      apply (fastforce dest: vs_lookup_slot_no_asid
+                       simp: ptes_of_Some pts_of_Some aobjs_of_Some obj_at_def)+
+  apply (erule state_vrefsD)
+    apply (fastforce simp: aobjs_of_Some obj_at_def)
+   apply clarsimp
+  apply (fastforce simp: vs_refs_aux_def graph_of_def pte_ref2_def split: if_splits)
+  done
 
 lemma mapM_x_swp_store_pte_pas_refined:
- "\<lbrace>pas_refined aag and invs and
-(\<lambda>s. \<forall>x \<in> set slots. table_base x \<notin> global_refs s \<and> (\<forall>asid. vspace_for_asid asid s \<noteq> Some (table_base x)))\<rbrace>
- mapM_x (swp store_pte InvalidPTE) slots
-\<lbrace>\<lambda>_ s. pas_refined aag s\<rbrace>"
-supply state_asids_to_policy_arch_def[simp del]
-apply (simp add: pas_refined_def)
-apply wpsimp
-apply (rule hoare_vcg_conj_lift, (wpsimp wp: mapM_x_wp_inv ; fail))+
-apply (wpsimp wp: store_pte_mapM_x_state_asids_to_policy store_pte_mapM_x_state_objs_in_policy)
-apply clarsimp
-done
+  "\<lbrace>pas_refined aag and invs and
+    (\<lambda>s. \<forall>x \<in> set slots. table_base x \<notin> global_refs s \<and>
+                         (\<forall>asid. vspace_for_asid asid s \<noteq> Some (table_base x)))\<rbrace>
+   mapM_x (swp store_pte InvalidPTE) slots
+   \<lbrace>\<lambda>_ s. pas_refined aag s\<rbrace>"
+  supply state_asids_to_policy_arch_def[simp del]
+  apply (rule hoare_strengthen_post)
+   apply (rule mapM_x_wp[where S="set slots"])
+    apply (simp add: pas_refined_def)
+    apply (wpsimp wp: store_pte_state_objs_in_policy store_pte_state_asids_to_policy
+                      store_pte_invs hoare_vcg_const_Ball_lift hoare_vcg_all_lift)
+    apply (auto simp: wellformed_pte_def)
+  done
 
 lemma dmo_state_vrefs[wp]:
   "do_machine_op f \<lbrace>\<lambda>s. P (state_vrefs s)\<rbrace>"
@@ -1643,49 +757,28 @@ lemma dmo_thread_states[wp]:
   "do_machine_op f \<lbrace>\<lambda>s. P (thread_states s)\<rbrace>"
   by (wpsimp wp: dmo_wp)
 
-
 lemma mapM_swp_store_pte_invs_unmap:
-  "\<lbrace>invs and
-    (\<lambda>s.  table_base p \<notin> global_refs s \<and>
-                        (\<forall>asid. vspace_for_asid asid s \<noteq> Some (table_base p))) and
-    K (pte = InvalidPTE)\<rbrace>
-  store_pte p pte \<lbrace>\<lambda>_. invs\<rbrace>"
-   apply simp
-   apply (wp store_pte_invs hoare_vcg_const_Ball_lift hoare_vcg_ex_lift hoare_vcg_all_lift)
-   apply (clarsimp simp: wellformed_pte_def)
-  done
-
-(* FIXME ryanb - use for simplifying some lemmas *)
-thm perform_pt_inv_unmap_invs
-
+  "\<lbrace>\<lambda>s. invs s \<and> pte = InvalidPTE \<and> table_base p \<notin> global_refs s
+               \<and> (\<forall>asid. vspace_for_asid asid s \<noteq> Some (table_base p))\<rbrace>
+   store_pte p pte
+   \<lbrace>\<lambda>_. invs\<rbrace>"
+  by (wpsimp wp: store_pte_invs simp: wellformed_pte_def)
 
 lemma FIXME_wordAND_wordNOT_mask_plus:
    "x && ~~mask n = x \<Longrightarrow> (x + mask n) && ~~mask n = x"
   by (metis AND_NOT_mask_plus_AND_mask_eq VSpaceEntries_AI.neg_mask_add_mask add_right_imp_eq word_bw_same(1))
 
-lemma table_base_mask:
-"p && ~~mask b = p \<Longrightarrow>
-       p' && ~~mask b = 0 \<Longrightarrow>
-       (p + p') && ~~mask b = p"
-  by (metis Groups.add_ac(2) VSpaceEntries_AI.neg_mask_add_mask add_left_imp_eq mask_eq_x_eq_0 word_plus_and_or_coroll2)
-
-
-
 lemma store_pte_pas_refined:
-  "\<lbrace>pas_refined aag and invs
-and (\<lambda>s. (\<exists>slot ref. caps_of_state s slot = Some (ArchObjectCap (PageTableCap (table_base p) ref)))
-\<and>  ((\<exists>asid. vspace_for_asid asid s = Some (table_base p)) \<longrightarrow> table_index p \<notin> kernel_mapping_slots) \<and>
-                table_base p \<notin> global_refs s
-)\<rbrace>
- store_pte p InvalidPTE
-\<lbrace>\<lambda>_. pas_refined aag\<rbrace>"
-supply state_asids_to_policy_arch_def[simp del]
-apply (clarsimp simp: pas_refined_def)
-apply (wpsimp wp: store_pte_state_objs_in_policy store_pte_state_asids_to_policy)
-done
+  "\<lbrace>\<lambda>s. pas_refined aag s \<and> invs s \<and> table_base p \<notin> global_refs s \<and>
+        (\<exists>slot ref. caps_of_state s slot = Some (ArchObjectCap (PageTableCap (table_base p) ref))) \<and>
+        ((\<exists>asid. vspace_for_asid asid s = Some (table_base p)) \<longrightarrow> table_index p \<notin> kernel_mapping_slots)\<rbrace>
+   store_pte p InvalidPTE
+   \<lbrace>\<lambda>_. pas_refined aag\<rbrace>"
+  supply state_asids_to_policy_arch_def[simp del]
+  apply (clarsimp simp: pas_refined_def)
+  apply (wpsimp wp: store_pte_state_objs_in_policy store_pte_state_asids_to_policy)
+  done
 
-
-(* FIXME ryanb: move *)
 lemma unmap_page_table_pas_refined:
  "\<lbrace>pas_refined aag and invs and K (vaddr \<in> user_region)\<rbrace>
   unmap_page_table asid vaddr pt
@@ -1700,12 +793,12 @@ lemma unmap_page_table_pas_refined:
    apply (fastforce dest: vs_lookup_slot_no_asid)
   apply (subst (asm) vs_lookup_slot_table_unfold; clarsimp)
   apply (intro conjI)
-    apply (frule vs_lookup_table_pt_at; clarsimp?)
-    apply (drule vs_lookup_table_valid_cap; clarsimp?)
-    apply (fastforce simp: valid_cap_def valid_arch_cap_def valid_arch_cap_ref_def obj_at_def
-                     dest: caps_of_state_valid split: cap.splits arch_cap.splits)
-   apply (metis vs_lookup_table_vspace user_region_slots is_aligned_neg_mask2 pt_slot_offset_offset)
-  apply (clarsimp simp: reachable_page_table_not_global)
+    apply (clarsimp simp: reachable_page_table_not_global)
+   apply (frule vs_lookup_table_pt_at; clarsimp?)
+   apply (drule vs_lookup_table_valid_cap; clarsimp?)
+   apply (fastforce simp: valid_cap_def valid_arch_cap_def valid_arch_cap_ref_def obj_at_def
+                    dest: caps_of_state_valid split: cap.splits arch_cap.splits)
+  apply (metis vs_lookup_table_vspace user_region_slots is_aligned_neg_mask2 pt_slot_offset_offset)
   done
 
 crunches unmap_page_table
@@ -1753,390 +846,251 @@ lemma perform_pt_inv_unmap_pas_refined:
   apply (clarsimp simp: is_cap_simps)
   done
 
+lemma vs_lookup_PageTablePTE:
+  "\<lbrakk> vs_lookup_table level asid vref s' = Some (lvl', pt);
+     pspace_aligned s; valid_vspace_objs s; valid_asid_table s;
+     invalid_pte_at p s; ptes_of s' = ptes_of s (p \<mapsto> pte); is_PageTablePTE pte;
+     asid_pools_of s' = asid_pools_of s; asid_table s' = asid_table s;
+     vref \<in> user_region;
+     pts_of s (the (pte_ref pte)) = Some empty_pt; pt \<noteq> pptr_from_pte pte \<rbrakk>
+     \<Longrightarrow> \<exists>level' \<ge> level. vs_lookup_table level' asid vref s = Some (lvl', pt)"
+  apply (induct level arbitrary: lvl' pt rule: bit0.from_top_full_induct[where y=max_pt_level])
+   apply (fastforce simp: geq_max_pt_level vs_lookup_table_def pool_for_asid_def obind_def)
+  apply (rule_tac x=lvl' in exI)
+  apply (frule vs_lookup_min_level, clarsimp)
+  apply (drule vs_lookup_level)
+  apply (case_tac "lvl' < max_pt_level")
+   apply (frule vs_lookup_table_split_last_Some; clarsimp)
+   apply (erule_tac x="lvl'+1" in allE)
+   apply (drule mp)
+    apply (fastforce elim: le_less_trans dest: vm_level_less_plus_1_mono)
+   apply (erule_tac x="lvl'+1" in allE)
+   apply clarsimp
+   apply (frule subst[where s="ptes_of s'" and P="\<lambda>ptes. ptes _ = _"])
+    apply assumption
+   apply (drule mp, fastforce simp: pte_ref_def2 ptes_of_Some split: if_splits)
+   apply (cases pte; clarsimp)
+   apply (drule_tac bot_level=level' in vs_lookup_level)
+   apply (subst vs_lookup_split_Some)
+     prefer 3
+     apply (rule exI, rule conjI, assumption)
+     apply (frule_tac P="\<lambda>x. x" and level1=lvl' and level'1="lvl'+1"
+                   in subst[OF vs_lookup_split_Some, rotated 2])
+       apply (fastforce dest: vm_level_less_le_1)
+      apply (fastforce dest: vm_level_less_max_pt_level vm_level_less_plus_1_mono)
+     apply clarsimp
+     apply (subst (asm) pt_walk.simps)
+     apply (clarsimp simp: obind_def)
+     apply (subst pt_walk.simps)
+     apply (clarsimp split: if_splits simp: obind_def)
+    apply (fastforce dest: vm_level_less_le_1)
+   apply (fastforce dest: vm_level_less_max_pt_level vm_level_less_plus_1_mono)
+  apply (case_tac "lvl' = asid_pool_level")
+   apply (auto simp: geq_max_pt_level vs_lookup_table_def pool_for_asid_def obind_def)
+  done
 
-
+lemma vs_lookup_PageTablePTE':
+  "\<lbrakk> vs_lookup_table level asid vref s = Some (lvl', pt);
+     pspace_aligned s; valid_vspace_objs s; valid_asid_table s;
+     invalid_pte_at p s; ptes_of s' = ptes_of s (p \<mapsto> pte); is_PageTablePTE pte;
+     asid_pools_of s' = asid_pools_of s; asid_table s' = asid_table s; vref \<in> user_region  \<rbrakk>
+     \<Longrightarrow> \<exists>level' \<ge> level. vs_lookup_table level' asid vref s' = Some (lvl', pt)"
+  apply (induct level arbitrary: lvl' pt rule: bit0.from_top_full_induct[where y=max_pt_level])
+   apply (fastforce simp: geq_max_pt_level vs_lookup_table_def pool_for_asid_def obind_def)
+  apply (rule_tac x=lvl' in exI)
+  apply (frule vs_lookup_min_level, clarsimp)
+  apply (drule vs_lookup_level)
+  apply (case_tac "lvl' < max_pt_level")
+   apply (frule vs_lookup_table_split_last_Some; clarsimp)
+   apply (erule_tac x="lvl'+1" in allE)
+   apply (drule mp)
+    apply (fastforce elim: le_less_trans dest: vm_level_less_plus_1_mono)
+   apply (erule_tac x="lvl'+1" in allE)
+   apply clarsimp
+   apply (drule_tac bot_level=level' in vs_lookup_level)
+   apply (subst vs_lookup_split_Some)
+     prefer 3
+     apply (rule exI, rule conjI, assumption)
+     apply (frule_tac P="\<lambda>x. x" and level1=lvl' and level'1="lvl'+1"
+                   in subst[OF vs_lookup_split_Some, rotated 2])
+       apply (fastforce dest: vm_level_less_le_1)
+      apply (fastforce dest: vm_level_less_max_pt_level vm_level_less_plus_1_mono)
+     apply clarsimp
+     apply (subst (asm) pt_walk.simps)
+     apply (clarsimp simp: obind_def split: if_splits)
+     apply (subst pt_walk.simps)
+     apply (clarsimp simp: obind_def split: if_splits)
+     apply (cases pte; clarsimp)
+     apply (frule is_aligned_pt[rotated])
+      apply (erule vs_lookup_table_pt_at; fastforce)
+     apply (clarsimp simp: invalid_pte_at_def ptes_of_Some pts_of_Some aobjs_of_Some)
+    apply (fastforce dest: vm_level_less_le_1)
+   apply (fastforce dest: vm_level_less_max_pt_level vm_level_less_plus_1_mono)
+  apply (case_tac "lvl' = asid_pool_level")
+   apply (auto simp: geq_max_pt_level vs_lookup_table_def pool_for_asid_def obind_def)
+  done
 
 lemma state_vrefs_store_PageTablePTE:
-  "\<lbrakk> invs s; is_aligned p pte_bits; vs_lookup_slot level asid vref s = Some (level, p);
-     vref \<in> user_region; is_PageTablePTE pte;  invalid_pte_at p s;
-     pts_of s (the (pte_ref pte)) = Some empty_pt; the (pte_ref pte) \<noteq> table_base p;
-     kheap s (table_base p) = Some (ArchObj (PageTable pt)) \<rbrakk>
-     \<Longrightarrow> state_vrefs (s\<lparr>kheap := \<lambda>a. if a = table_base p
-                                     then Some (ArchObj (PageTable (\<lambda>a. if a = table_index p then pte else pt a)))
+  assumes "invs s"
+  and "is_aligned p pte_bits"
+  and "vs_lookup_slot level asid vref s = Some (level, p)"
+  and "vref \<in> user_region"
+  and "is_PageTablePTE pte"
+  and "invalid_pte_at p s"
+  and "pts_of s (the (pte_ref pte)) = Some empty_pt"
+  and "the (pte_ref pte) \<noteq> table_base p"
+  and "kheap s (table_base p) = Some (ArchObj (PageTable pt))"
+  shows "state_vrefs (s\<lparr>kheap := \<lambda>a. if a = table_base p
+                                     then Some (ArchObj (PageTable (\<lambda>a. if a = table_index p
+                                                                        then pte
+                                                                        else pt a)))
                                      else kheap s a\<rparr>) =
          (\<lambda>x. if x = table_base p
               then vs_refs_aux level (PageTable (\<lambda>a. if a = table_index p then pte else pt a))
               else state_vrefs s x)"
+  (is "state_vrefs ?s' = _")
+  using assms
+  apply -
   apply (rule all_ext)
-
   apply (case_tac "level = asid_pool_level")
-     apply (clarsimp simp: vs_lookup_slot_def split: if_splits)
-     apply (clarsimp simp: vs_lookup_table_def split: if_splits)
-     apply (drule pool_for_asid_no_pte)
-        apply (simp add: ptes_of_Some pts_of_Some aobjs_of_Some)
-       apply fastforce
-      apply fastforce
-     apply fastforce
-
-apply safe
-
-
-(* first thing *)
-
+   apply (fastforce simp: vs_lookup_slot_def vs_lookup_table_def
+                          ptes_of_Some pts_of_Some aobjs_of_Some
+                    dest: pool_for_asid_no_pte split: if_splits)
+  apply safe
    apply (clarsimp simp: state_vrefs_def opt_map_def split: option.splits)
    apply (case_tac "x = pptr_from_pte pte")
-    (* x = pptr_from_pte pte *)
-  apply clarsimp
-    apply (clarsimp simp: pte_ref_def2)
-    apply (clarsimp split: if_splits)
-    apply (clarsimp simp: vs_refs_aux_def graph_of_def pte_ref2_def)
-      (* x \<noteq> pptr_from_pte pte *)
-   apply (drule_tac s=s and pte=pte and p=p in vs_lookup_PageTablePTE[rotated 9])
-    (* discharging above *)
-               apply (clarsimp simp: pts_of_Some aobjs_of_Some)
-              apply fastforce+
-        apply (rule all_ext)
-        apply (clarsimp simp: opt_map_def pte_of_def obind_def)
-        apply (fastforce dest: pte_ptr_eq)
-       apply simp
-      apply (fastforce simp: opt_map_def)
-     apply (fastforce simp: opt_map_def)
-    apply clarsimp
-(* done *)
+    apply (clarsimp simp: pte_ref_def2 split: if_splits)
+    apply (fastforce simp: vs_refs_aux_def graph_of_def pte_ref2_def)
+   apply (drule_tac s=s and pte=pte and p=p in vs_lookup_PageTablePTE)
+              apply (fastforce simp: pts_of_Some aobjs_of_Some opt_map_def pte_of_def obind_def
+                               dest: pte_ptr_eq)+
    apply clarsimp
    apply (drule vs_lookup_level)
    apply (case_tac "lvl = asid_pool_level")
-    (* lvla = asid_pool_level *)
-    apply clarsimp
-    apply (frule vs_lookup_asid_pool)
-     apply fastforce
-    apply (fastforce simp: asid_pools_of_ko_at obj_at_def)
-    (* lvla \<noteq> asid_pool_level *)
-   apply clarsimp
-   apply (frule vs_lookup_table_pt_at)
-        apply fastforce+
-   apply (clarsimp simp: typ_at_eq_kheap_obj)
-   apply (case_tac "x = table_base p"; clarsimp)
-
-
-    apply (subst (asm) vs_lookup_slot_table)
-     apply clarsimp
-    apply clarsimp
-    apply (prop_tac "is_aligned pt_ptr pt_bits")
-     apply (rule is_aligned_pt[rotated])
-      apply fastforce
-     apply (erule vs_lookup_table_pt_at; fastforce)
-    apply clarsimp
-    apply (drule (1) vs_lookup_table_unique_level; fastforce)
-    (* x \<noteq> table_base p *)
-   apply fastforce
-
-(* second thing *)
-
+    apply (fastforce dest: vs_lookup_asid_pool  simp: asid_pools_of_ko_at obj_at_def)
+   apply (subst (asm) vs_lookup_slot_table_unfold; clarsimp)
+   apply (fastforce dest: vs_lookup_table_unique_level split: if_splits)
   apply (clarsimp simp: state_vrefs_def opt_map_def)
-
-
-   apply (frule vs_lookup_slot_table_base)
-      apply clarsimp+
-
-   apply (case_tac "x = table_base p"; clarsimp)
-
-   apply (drule_tac pte=pte and s'="(s\<lparr>kheap :=
-                                 \<lambda>a. if a = table_base p
-                                      then Some (ArchObj (PageTable (\<lambda>a. if a = table_index p then pte else pt a)))
-                                      else kheap s a\<rparr>)" in vs_lookup_PageTablePTE'[rotated 9])
-            apply fastforce+
-        apply (rule all_ext)
-        apply (clarsimp simp: opt_map_def pte_of_def obind_def)
-        apply (fastforce dest: pte_ptr_eq)
-       apply simp
-      apply (fastforce simp: opt_map_def)
-     apply (fastforce simp: opt_map_def)
-    apply clarsimp
-   apply fastforce
-
-  apply (drule_tac pte=pte and s'="(s\<lparr>kheap :=
-                                \<lambda>a. if a = table_base p
-                                     then Some (ArchObj (PageTable (\<lambda>a. if a = table_index p then pte else pt a)))
-                                     else kheap s a\<rparr>)" in vs_lookup_PageTablePTE'[rotated 9]) back
-           apply fastforce+
-       apply (rule all_ext)
-       apply (clarsimp simp: opt_map_def pte_of_def obind_def)
-       apply (fastforce dest: pte_ptr_eq)
-      apply simp
-     apply (fastforce simp: opt_map_def)
-    apply (fastforce simp: opt_map_def)
-   apply clarsimp
-  apply fastforce
+  apply (frule vs_lookup_slot_table_base)
+     apply clarsimp+
+  apply (case_tac "x = table_base p"; clarsimp)
+   apply (drule_tac pte=pte and s'="?s'" in vs_lookup_PageTablePTE';
+          fastforce dest: pte_ptr_eq simp: pts_of_Some aobjs_of_Some opt_map_def pte_of_def obind_def)
+  apply (drule_tac level=bot and pte=pte and s'="?s'" in vs_lookup_PageTablePTE';
+         fastforce dest: pte_ptr_eq simp: pts_of_Some aobjs_of_Some opt_map_def pte_of_def obind_def)
   done
-
 
 lemma state_vrefs_store_PageTablePTE_wp:
-"\<lbrace>\<lambda>s. invs s \<and> is_PageTablePTE pte \<and> invalid_pte_at p s \<and>
-pts_of s (the (pte_ref pte)) = Some empty_pt \<and> the (pte_ref pte) \<noteq> table_base p \<and>
-(\<exists>level asid vref. vs_lookup_slot level asid vref s = Some (level, p) \<and> vref \<in> user_region \<and>
-(\<forall>pt. ako_at (PageTable pt) (table_base p) s \<longrightarrow>
-P (\<lambda>x. if x = table_base p
-                   then vs_refs_aux level (PageTable (\<lambda>a. if a = table_index p then pte else pt a))
-                   else state_vrefs s x)))
-\<rbrace> store_pte p pte \<lbrace>\<lambda>_ s. P (state_vrefs s)\<rbrace>"
-unfolding store_pte_def set_pt_def
-apply (wpsimp wp: set_object_wp)
-apply (clarsimp simp: fun_upd_def)
-apply (subst state_vrefs_store_PageTablePTE)
-apply fastforce+
-apply (clarsimp simp: obj_at_def)
-apply clarsimp
-done
-
-
-
-
-lemma perform_pt_inv_map_pas_refined[wp]:
-"\<lbrace>pas_refined aag and invs and valid_pti (PageTableMap acap (a, b) pte p)
-and K (authorised_page_table_inv aag (PageTableMap acap (a, b) pte p))\<rbrace>
-            perform_pt_inv_map acap (a,b) pte p
-            \<lbrace>\<lambda>_. pas_refined aag\<rbrace>"
-  unfolding perform_pt_inv_map_def
-  apply (rule hoare_gen_asm)
-  apply wpsimp
-    apply (clarsimp simp: pas_refined_def state_objs_to_policy_def)
-   apply (wps | wpsimp wp: state_vrefs_store_PageTablePTE_wp arch_update_cap_invs_map  vs_lookup_slot_lift
-                     hoare_vcg_ex_lift hoare_vcg_all_lift hoare_vcg_imp_lift' set_cap_arch_obj_neg set_cap_state_vrefs)+
-
-
-  apply (clarsimp simp: valid_pti_def)
-  apply (clarsimp simp: conj_ac )
-  apply (case_tac acap; clarsimp)
-  apply (intro conjI impI)
-     apply (clarsimp simp: cte_wp_at_caps_of_state)
-     apply (clarsimp simp: is_arch_update_def is_arch_cap_def cap_master_cap_def)
-     apply (prop_tac "valid_cap cap s")
-      apply (rule cte_wp_valid_cap)
-       apply (fastforce simp: cte_wp_at_caps_of_state)
-      apply fastforce
-     apply (case_tac cap; clarsimp)
-     apply (case_tac x12; clarsimp)
-     apply (case_tac x42; clarsimp)
-     apply (clarsimp simp: valid_cap_def cap_aligned_def valid_arch_cap_def)
-
-    apply clarsimp
-    apply (clarsimp simp: vs_lookup_slot_def split: if_splits)
-
-     apply (clarsimp simp: vs_lookup_table_def)
-     apply (clarsimp simp: invalid_pte_at_def)
-     apply (drule pool_for_asid_no_pte)
-        apply (simp)
-       apply fastforce
-      apply fastforce
-     apply simp
-
-    apply clarsimp
-
-    apply (prop_tac "is_aligned ba pt_bits")
-     apply (drule (2) vs_lookup_table_is_aligned)
-        apply fastforce
-       apply fastforce
-      apply fastforce
-     apply clarsimp
-    apply (rename_tac vref' ao pt')
-    apply clarsimp
-    apply (drule (1) vs_lookup_table_target)
-    apply (drule valid_vs_lookupD, erule vref_for_level_user_region; clarsimp)
-    apply (prop_tac "is_pt_cap cap")
-     apply (erule_tac s=s in valid_cap_to_pt_cap[rotated])
-  using pt_at_eq apply blast
-     apply (rule cte_wp_valid_cap)
-      apply (fastforce simp: cte_wp_at_caps_of_state)
-     apply fastforce
-
-    apply (frule (1) cap_to_pt_is_pt_cap, simp, fastforce intro: valid_objs_caps)
-    apply (clarsimp simp: is_cap_simps)
-    apply (clarsimp simp: cte_wp_at_caps_of_state)
-    apply (clarsimp simp: is_arch_update_def cap_master_cap_def split: cap.splits arch_cap.splits option.splits)
-
-    apply (drule (1) unique_table_refsD[rotated])
-      apply clarsimp
-     apply fastforce
-    apply (clarsimp simp: table_cap_ref_def)
-
-   apply (erule cte_wp_at_weakenE)
-   apply clarsimp
-   apply (case_tac c; clarsimp)
-   apply (clarsimp simp: vs_cap_ref_def vs_cap_ref_arch_def split: arch_cap.splits)
-   apply (clarsimp simp: is_arch_update_def cap_master_cap_def)
-
-
-  apply (rule_tac x=level in exI)
-  apply (rename_tac asid ao)
-  apply (rule_tac x=asid in exI)
-  apply (rule_tac x=vref in exI)
-  apply clarsimp
-
-  apply (intro conjI impI; (fastforce | (clarsimp simp: pas_refined_def; fail))?)
-       apply clarsimp
-  using Invariants_AI.cte_wp_at_cte_at apply blast
-
-      apply clarsimp
-      apply (erule state_asids_to_policy_aux.cases)
-  using Invariants_AI.cte_wp_at_cte_at apply blast
-  using Invariants_AI.cte_wp_at_cte_at apply blast
-  using Invariants_AI.cte_wp_at_cte_at apply blast
-  using Invariants_AI.cte_wp_at_cte_at apply blast
-
-    apply (clarsimp split: if_splits)
-    apply (clarsimp simp: pas_refined_def)
-    apply (erule state_irqs_to_policy_aux.cases)
-    apply (clarsimp split: if_splits)
-    apply (fastforce dest: sita_controlled)
-
-(* state_asids_to_policy *)
-   apply clarsimp
-   apply (erule state_asids_to_policy_aux.cases)
-
-     apply (clarsimp simp: cte_wp_at_caps_of_state)
-     apply (clarsimp split: if_splits)
-
-      apply (clarsimp simp: authorised_page_table_inv_def)
-      apply (clarsimp simp: aag_cap_auth_def cap_auth_conferred_def arch_cap_auth_conferred_def cap_links_asid_slot_def label_owns_asid_slot_def)
-     apply (clarsimp simp: pas_refined_def)
-     apply (erule subsetD) back
-  thm sata_asid
-     apply (fastforce dest: sata_asid)
-    apply clarsimp
-    apply (clarsimp split: if_splits)
-     prefer 2
-     apply (fastforce simp: pas_refined_def dest: subsetD dest!: sata_asid_lookup)
-    apply (clarsimp simp: vs_refs_aux_def)
-   apply (fastforce simp: pas_refined_def dest: subsetD dest!: state_asids_to_policy_aux.intros)
-
-  apply clarsimp
-  apply (clarsimp simp: cte_wp_at_caps_of_state)
-  apply (clarsimp simp: auth_graph_map_def)
-  apply (erule state_bits_to_policy.cases)
-    (* sbta_caps *)
-        apply (clarsimp simp: pas_refined_def is_arch_update_def cap_master_cap_def
-                              auth_graph_map_def state_objs_to_policy_def
-                       split: if_splits cap.splits arch_cap.splits option.splits;
-               fastforce dest: sbta_caps simp: cap_auth_conferred_def arch_cap_auth_conferred_def)
-    (* sbta_untyped *)
-        apply (clarsimp simp: pas_refined_def is_arch_update_def cap_master_cap_def
-                              auth_graph_map_def state_objs_to_policy_def
-                       split: if_splits cap.splits arch_cap.splits option.splits;
-               fastforce dest: sbta_untyped simp: cap_auth_conferred_def arch_cap_auth_conferred_def)
-    (* sbta_ts *)
-        apply (clarsimp simp: pas_refined_def is_arch_update_def cap_master_cap_def
-                              auth_graph_map_def state_objs_to_policy_def
-                       split: if_splits cap.splits arch_cap.splits option.splits;
-               fastforce dest: sbta_ts simp: cap_auth_conferred_def arch_cap_auth_conferred_def)
-    (* sbta_bounds *)
-        apply (clarsimp simp: pas_refined_def is_arch_update_def cap_master_cap_def
-                              auth_graph_map_def state_objs_to_policy_def
-                       split: if_splits cap.splits arch_cap.splits option.splits;
-               fastforce dest: sbta_bounds simp: cap_auth_conferred_def arch_cap_auth_conferred_def)
-    (* sbta_cdt *)
-    apply (clarsimp simp: is_arch_update_def cap_master_cap_def split: cap.splits arch_cap.splits option.splits)
-    apply (clarsimp simp: pas_refined_def)
-    apply (erule subsetD)
-    apply (clarsimp simp: auth_graph_map_def state_objs_to_policy_def)
-    apply (clarsimp split: if_splits)
-     apply (rule exI, rule conjI, rule refl)+
-     apply (drule_tac caps="caps_of_state s" in sbta_cdt)
-      apply simp
-      apply clarsimp
-      apply (fastforce elim: is_transferable.cases)
-     apply fastforce
-    apply (rule exI, rule conjI, rule refl)+
-    apply (drule_tac caps="caps_of_state s" in sbta_cdt)
-     apply simp
-    apply clarsimp
-    apply (fastforce elim: is_transferable.cases)
-    (* sbta_cdt_transferable *)
-   apply (clarsimp simp: is_arch_update_def cap_master_cap_def split: cap.splits arch_cap.splits option.splits)
-   apply (clarsimp simp: pas_refined_def)
-   apply (erule subsetD)
-   apply (clarsimp simp: auth_graph_map_def state_objs_to_policy_def)
-   apply (fastforce dest: sbta_cdt_transferable)
-    (* sbta_vref *)
-  apply (clarsimp split: if_splits)
-   prefer 2
-   apply (clarsimp simp: is_arch_update_def cap_master_cap_def split: cap.splits arch_cap.splits option.splits)
-   apply (clarsimp simp: pas_refined_def)
-   apply (erule subsetD)
-   apply (clarsimp simp: auth_graph_map_def state_objs_to_policy_def)
-   apply (fastforce dest: sbta_vref)
-
-  apply (clarsimp simp: authorised_page_table_inv_def)
-
-apply (simp only: vs_refs_aux_def arch_kernel_obj.case)
-apply clarsimp
-
-apply (case_tac "level \<noteq> max_pt_level \<or> aa \<notin> kernel_mapping_slots"; clarsimp simp: word_le_not_less)
-
-apply (subgoal_tac "(pasSubject aag, baa, pasObjectAbs aag ac) \<in> pasPolicy aag")
-apply clarsimp
-apply (thin_tac "_ \<notin> _")
-
-  apply (clarsimp simp: vs_refs_aux_def graph_of_def)
-
-apply (subgoal_tac "(pasSubject aag, baa, pasObjectAbs aag ac) \<in> pasPolicy aag")
-apply clarsimp
-
-  apply (case_tac pte; clarsimp)
-  apply (clarsimp simp: pte_ref2_def aag_cap_auth_def cap_auth_conferred_def arch_cap_auth_conferred_def)
-  apply (case_tac "aa = table_index p"; clarsimp)
-
-
-  apply (clarsimp simp: is_arch_update_def cap_master_cap_def split: cap.splits arch_cap.splits option.splits)
-  apply (clarsimp simp: pas_refined_def)
-  apply (erule subsetD)
-  apply (clarsimp simp: auth_graph_map_def state_objs_to_policy_def)
-  apply (rule_tac x="table_base p" in exI, rule conjI)
-   apply simp
-  apply (rule exI, rule conjI, rule refl)
-  apply (rule sbta_vref)
-  apply (clarsimp simp: state_vrefs_def)
-  thm sbta_vref
-
-  apply (case_tac "level = asid_pool_level")
-   apply (clarsimp simp: vs_lookup_slot_def split: if_splits)
-
-   apply (clarsimp simp: vs_lookup_table_def)
-   apply (clarsimp simp: invalid_pte_at_def)
-   apply (drule pool_for_asid_no_pte)
-      apply (simp)
-     apply fastforce
-    apply fastforce
-   apply simp
-
-  apply clarsimp
-  apply (drule vs_lookup_slot_table_base)
-     apply clarsimp+
-
-  apply (rule exI, rule conjI)
-   apply (rule exI, rule exI)
-   apply (rule conjI, rule refl)
-   apply (rule exI)+
-   apply (rule conjI, assumption)
-   apply (simp add: obj_at_def aobjs_of_Some)
-  apply (clarsimp simp: vs_refs_aux_def graph_of_def)
-  apply (clarsimp simp: pte_ref2_def)
-  apply fastforce
+  "\<lbrace>\<lambda>s. invs s \<and> is_PageTablePTE pte \<and> invalid_pte_at p s \<and>
+        pts_of s (the (pte_ref pte)) = Some empty_pt \<and> the (pte_ref pte) \<noteq> table_base p \<and>
+        (\<exists>level asid vref. vs_lookup_slot level asid vref s = Some (level, p) \<and> vref \<in> user_region \<and>
+                           (\<forall>pt. ako_at (PageTable pt) (table_base p) s \<longrightarrow>
+                                 P (\<lambda>x. if x = table_base p
+                                        then vs_refs_aux level (PageTable (\<lambda>a. if a = table_index p
+                                                                               then pte
+                                                                               else pt a))
+                                        else state_vrefs s x)))\<rbrace>
+   store_pte p pte
+   \<lbrace>\<lambda>_ s. P (state_vrefs s)\<rbrace>"
+  unfolding store_pte_def set_pt_def
+  apply (wpsimp wp: set_object_wp)
+  apply (fastforce simp: fun_upd_def obj_at_def state_vrefs_store_PageTablePTE)
   done
 
+lemma perform_pt_inv_map_pas_refined[wp]:
+  "\<lbrace>pas_refined aag and invs and valid_pti (PageTableMap acap (a, b) pte p)
+                    and K (authorised_page_table_inv aag (PageTableMap acap (a, b) pte p))\<rbrace>
+   perform_pt_inv_map acap (a,b) pte p
+   \<lbrace>\<lambda>_. pas_refined aag\<rbrace>"
+  unfolding perform_pt_inv_map_def
+  apply (rule hoare_gen_asm)
+  apply (wpsimp simp: pas_refined_def state_objs_to_policy_def)
+    apply (wps | wpsimp wp: state_vrefs_store_PageTablePTE_wp arch_update_cap_invs_map
+                            vs_lookup_slot_lift set_cap_arch_obj_neg set_cap_state_vrefs
+                            hoare_vcg_ex_lift hoare_vcg_all_lift hoare_vcg_imp_lift')+
+  apply (clarsimp simp: invs_psp_aligned invs_vspace_objs invs_arch_state
+                        valid_pti_def cte_wp_at_cte_at)
+  apply (case_tac acap; clarsimp)
+  apply (intro conjI; (solves \<open>simp add: pas_refined_def\<close>)?)
+     apply (fastforce simp: cte_wp_at_caps_of_state vs_cap_ref_def
+                            is_arch_update_def cap_master_cap_def
+                     split: arch_cap.splits)
+    apply (clarsimp simp: cte_wp_at_caps_of_state)
+    apply (fastforce dest: caps_of_state_valid
+                    simp: vs_cap_ref_def is_arch_update_def cap_master_cap_def
+                          valid_cap_def cap_aligned_def valid_arch_cap_def
+                   split: cap.splits arch_cap.splits)
+   apply (clarsimp simp: vs_lookup_slot_def split: if_splits)
+    apply (fastforce dest: pool_for_asid_no_pte simp: vs_lookup_table_def invalid_pte_at_def)
+   apply (frule (2) vs_lookup_table_is_aligned; clarsimp)
+   apply (drule (1) vs_lookup_table_target)
+   apply (drule valid_vs_lookupD, erule vref_for_level_user_region; clarsimp)
+   apply (frule (1) cap_to_pt_is_pt_cap, simp, fastforce intro: valid_objs_caps)
+   apply (clarsimp simp: cte_wp_at_caps_of_state)
+   apply (clarsimp simp: is_cap_simps is_arch_update_def cap_master_cap_def
+                  split: cap.splits arch_cap.splits)
+   apply (drule (1) unique_table_refsD[rotated]; fastforce simp: table_cap_ref_def)
+  apply (intro exI conjI; (simp | clarsimp))
+  apply (intro conjI)
+    apply (clarsimp simp: pas_refined_def cte_wp_at_caps_of_state auth_graph_map_def)
+    apply (erule state_bits_to_policy.cases)
+          apply (clarsimp simp: is_arch_update_def cap_master_cap_def state_objs_to_policy_def
+                         split: if_splits cap.splits arch_cap.splits option.splits;
+                 fastforce dest: sbta_caps simp: cap_auth_conferred_def arch_cap_auth_conferred_def)
+         apply (fastforce dest: sbta_untyped simp: state_objs_to_policy_def split: if_splits)
+        apply (fastforce dest: sbta_ts simp: state_objs_to_policy_def)
+       apply (fastforce dest: sbta_bounds simp: state_objs_to_policy_def)
+      apply (clarsimp simp: state_objs_to_policy_def is_arch_update_def cap_master_cap_def)
+      apply (drule_tac caps="caps_of_state s" in sbta_cdt; fastforce elim: is_transferable.cases
+                                                                    split: if_splits)
+     apply (fastforce dest: sbta_cdt_transferable simp: state_objs_to_policy_def)
+    apply (clarsimp split: if_splits)
+     apply (clarsimp simp: authorised_page_table_inv_def vs_refs_aux_def split: arch_kernel_obj.splits)
+     apply (erule swap)
+     apply (clarsimp simp: graph_of_def pte_ref2_def split: if_split_asm)
+      apply (cases pte; clarsimp simp: aag_cap_auth_def cap_auth_conferred_def arch_cap_auth_conferred_def)
+     apply (erule subsetD)
+     apply (clarsimp simp: auth_graph_map_def state_objs_to_policy_def)
+     apply (rule_tac x="table_base p" in exI, rule conjI, erule sym)
+     apply (rule exI, rule conjI, rule refl)
+     apply (rule sbta_vref)
+     apply (case_tac "level = asid_pool_level")
+      apply (fastforce dest: pool_for_asid_no_pte
+                       simp: vs_lookup_slot_def vs_lookup_table_def invalid_pte_at_def)
+     apply (subst (asm) vs_lookup_slot_table_unfold; clarsimp)
+     apply (erule state_vrefsD)
+       apply (fastforce simp: aobjs_of_Some obj_at_def)
+      apply clarsimp
+     apply (fastforce simp: vs_refs_aux_def graph_of_def pte_ref2_def)
+    apply (clarsimp simp: is_arch_update_def cap_master_cap_def
+                   split: cap.splits arch_cap.splits option.splits)
+    apply (fastforce dest: sbta_vref simp: pas_refined_def auth_graph_map_def state_objs_to_policy_def)
+   apply (clarsimp simp: pas_refined_def)
+   apply (erule state_asids_to_policy_aux.cases)
+     apply (clarsimp simp: cte_wp_at_caps_of_state split: if_splits)
+      apply (clarsimp simp: authorised_page_table_inv_def aag_cap_auth_def
+                            cap_auth_conferred_def arch_cap_auth_conferred_def
+                            cap_links_asid_slot_def label_owns_asid_slot_def)
+     apply (fastforce dest: sata_asid)
+    apply (clarsimp split: if_splits)
+     apply (fastforce dest!: state_asids_to_policy_aux.intros simp: vs_refs_aux_def)
+    apply (fastforce dest!: sata_asid_lookup)
+   apply (fastforce dest!: sata_asidpool)
+  apply (clarsimp simp: pas_refined_def)
+  apply (erule state_irqs_to_policy_aux.cases)
+  apply (clarsimp split: if_splits)
+  apply (fastforce dest: sita_controlled)
+  done
 
-
-(* FIXME ryanb: resume *)
 lemma perform_page_table_invocation_pas_refined:
-  "\<lbrace>pas_refined aag and invs and valid_pti iv
-and K (authorised_page_table_inv aag iv)\<rbrace> perform_page_table_invocation iv \<lbrace>\<lambda>_. pas_refined aag\<rbrace>"
-unfolding perform_page_table_invocation_def
-apply wpsimp
-apply (wpsimp wp: perform_pt_inv_unmap_pas_refined perform_pt_inv_map_pas_refined)+
-apply (case_tac iv; clarsimp)
-done
-
-
+  "\<lbrace>pas_refined aag and invs and valid_pti iv and K (authorised_page_table_inv aag iv)\<rbrace>
+   perform_page_table_invocation iv
+   \<lbrace>\<lambda>_. pas_refined aag\<rbrace>"
+  unfolding perform_page_table_invocation_def
+  apply wpsimp
+   apply (wpsimp wp: perform_pt_inv_unmap_pas_refined perform_pt_inv_map_pas_refined)+
+  apply (case_tac iv; clarsimp)
+  done
 
 lemma auth_graph_map_def2:
   "auth_graph_map f S = (\<lambda>(x, auth, y). (f x, auth, f y)) ` S"
@@ -2149,19 +1103,6 @@ lemma store_pte_ekheap[wp]:
   apply (wp get_object_wp)
   apply simp
   done
-
-
-lemma set_asid_pool_st_vrefs[wp]:
-  "\<lbrace>\<lambda>s. P ((state_vrefs s) (p := (\<lambda>(r, p). (p, ucast r, AASIDPool, Control)) ` graph_of pool))\<rbrace>
-   set_asid_pool p pool
-   \<lbrace>\<lambda>rv s. P (state_vrefs s)\<rbrace>"
-  apply (simp add: set_asid_pool_def set_object_def)
-  apply (wp get_object_wp)
-  apply (clarsimp simp: state_vrefs_def fun_upd_def[symmetric] fun_upd_comp obj_at_def
-                        vs_refs_aux_def
-                 split: kernel_object.split_asm arch_kernel_obj.split_asm
-                 elim!: rsubst[where P=P, OF _ ext])
-  oops
 
 lemma set_asid_pool_thread_states[wp]:
   "set_asid_pool p pool \<lbrace>\<lambda>s. P (thread_states s)\<rbrace>"
@@ -2187,48 +1128,6 @@ lemma set_asid_pool_ekheap[wp]:
   apply (simp add: set_asid_pool_def)
   apply (wp get_object_wp | simp)+
   done
-
-lemma set_asid_pool_pas_refined[wp]:
-  "\<lbrace>pas_refined aag and
-    (\<lambda>s. \<forall>(x, y) \<in> graph_of pool.
-           auth_graph_map (pasObjectAbs aag) {(p, Control, y)} \<subseteq> pasPolicy aag \<and>
-           (\<forall>asid. asid_table s (asid_high_bits_of asid) = Some p \<and>
-                   asid && mask asid_low_bits = ucast x
-                   \<longrightarrow> (pasASIDAbs aag asid, Control, pasObjectAbs aag y) \<in> pasPolicy aag))\<rbrace>
-         set_asid_pool p pool \<lbrace>\<lambda>rv. pas_refined aag\<rbrace>"
-  apply (simp add: auth_graph_map_def2 image_UN split_def)
-  apply (simp add: pas_refined_def state_objs_to_policy_def)
-  apply (rule hoare_pre)
-   apply (wp tcb_domain_map_wellformed_lift | wps)+
-(*
-  apply clarsimp
-  apply (rule conjI)
-   apply (clarsimp dest!: auth_graph_map_memD)
-   apply (erule state_bits_to_policy.cases,
-          auto intro: state_bits_to_policy.intros auth_graph_map_memI
-               split: if_split_asm)[1]
-  apply (auto intro: state_asids_to_policy_aux.intros
-               simp: subsetD[OF _ state_asids_to_policy_aux.intros(2)]
-              elim!: state_asids_to_policy_aux.cases
-              split: if_split_asm)
-*)
-  oops
-(* FIXME ryanb
-  apply fastforce+
-  done
-*)
-
-lemma pas_refined_clear_asid:
-  "pas_refined aag s
-   \<Longrightarrow> pas_refined aag (s\<lparr>arch_state := arch_state s\<lparr>riscv_asid_table := \<lambda>a. if a = asid then None
-                                                                             else asid_table s a\<rparr>\<rparr>)"
-  oops
-(* FIXME ryanb
-  by (fastforce simp: pas_refined_def state_objs_to_policy_def
-               intro: state_asids_to_policy_aux.intros
-               elim!: state_asids_to_policy_aux.cases
-               split: if_split_asm)
-*)
 
 crunch integrity_autarch: set_asid_pool "integrity aag X st"
   (wp: crunch_wps)
